theories/Datatype/PairLevel.v
@@ -1,56 +1,56 @@
 From Coq Require Import Orders Lia RelationPairs Bool.Bool Structures.EqualitiesFacts.
 From DeBrLevel Require Import LevelInterface Level.
 
+(** * Implementation - Pair 
+
+  Implementation of leveled elements embedded in a pair type. We use the notation [ET] when elements satisfy [Equality Type] module, [OT] when elements satisfy [Ordered Type] module, [WL] when the embedded type has an equivalent equality to the one from Coq, [FL] when the embbeded type has boolean version of [Wf] and finally [BD] when elements does not contains binders associated to levels.
+*)
+
+(** ** Leveled Pair Implementation - [ET] *)
 Module IsLvlPairET (O1 : IsLvlET) (O2 : IsLvlET) <: IsLvlET.
 
-(** *** Definition *)
-Section definition.
-Definition t := (O1.t * O2.t)%type.
+(** *** Definitions *)
 
+Definition t := (O1.t * O2.t)%type.
 Definition eq := (O1.eq * O2.eq)%signature.
 
-#[global]
-Instance eq_equiv : Equivalence eq := _.
+Definition shift (m n : Lvl.t) (t : t) := 
+  (O1.shift m n (fst t),O2.shift m n (snd t)).
 
-Definition shift (lb k : Level.t) (t : t) := 
-  (O1.shift lb k (fst t),O2.shift lb k (snd t)).
+Definition Wf (m : Lvl.t) (t : t) := 
+  (O1.Wf m (fst t)) /\ ((O2.Wf m) (snd t)).
 
-Definition valid (lb : Level.t) (t : t) := 
-  (O1.valid lb (fst t)) /\ ((O2.valid lb) (snd t)).
+(** *** Properties *)
 
-End definition.
+(** **** [eq] properties *)
 
-(** *** Equality *)
-Section equality.
 
-Lemma eq_refl : Reflexive eq. 
-Proof. 
-  red; intros; destruct x; unfold eq; split;
-  unfold RelationPairs.RelCompFun; simpl; reflexivity.
-Qed.
+#[export] Instance eq_refl : Reflexive eq := _. 
+#[export] Instance eq_sym  : Symmetric eq := _.
+#[export] Instance eq_trans : Transitive eq := _.
 
-Lemma eq_sym  : Symmetric eq.
-Proof. 
-  red; intros; destruct x,y; unfold eq in *; split; destruct H;
-  unfold RelationPairs.RelCompFun in *; simpl in *; now symmetry.
-Qed.
+#[export] Instance eq_equiv : Equivalence eq := _.
 
-Lemma eq_trans : Transitive eq.
-Proof. 
-  red; intros; destruct x,y,z; unfold eq in *; split; destruct H,H0;
-  unfold RelationPairs.RelCompFun in *; simpl in *; etransitivity; eauto.
-Qed.
 
-#[export]
-Instance shift_eq : Proper (Logic.eq ==> Logic.eq ==> eq ==> eq) shift.
+(** **** [shift] properties *)
+Section shift.
+
+Variable m n k p : Lvl.t.
+Variable t : t.
+
+#[export] Instance shift_eq : Proper (Logic.eq ==> Logic.eq ==> eq ==> eq) shift.
 Proof.
-  repeat red; intros; subst; destruct x1,y1.
-  destruct H1; unfold RelationPairs.RelCompFun in *; simpl in *;
-  split; try (now apply O1.shift_eq); now apply O2.shift_eq.
+  clear; intros m' m Heqm n' n Heqn t t' Heq; subst.
+  destruct t as [ft st]; destruct t' as [ft' st'].
+  destruct Heq as [Hfeq Hseq].
+  unfold eq, shift, RelationPairs.RelCompFun in *; simpl in *.
+  split; red; simpl.
+  - now apply O1.shift_eq.
+  - now apply O2.shift_eq.
 Qed.
 
-Lemma shift_eq_iff : forall lb k t t1, 
-  eq t t1 <-> eq (shift lb k t) (shift lb k t1).
+Lemma shift_eq_iff : forall m n t t1, 
+  eq t t1 <-> eq (shift m n t) (shift m n t1).
 Proof.
   split; intro Heq; destruct t0,t1,Heq; split;
   unfold RelationPairs.RelCompFun in *; simpl in *.
@@ -60,51 +60,33 @@ Proof.
   - rewrite O2.shift_eq_iff; eauto.
 Qed.
 
-#[export]
-Instance valid_eq : Proper (Logic.eq ==> eq ==> iff) valid.
-Proof.
-  repeat red; intros; subst; destruct x0,y0,H0.
-  unfold RelationPairs.RelCompFun in *; simpl in *.
-  split; intros; destruct H1; split; simpl in *;
-  try (eapply O1.valid_eq; eauto; now symmetry);
-  eapply O2.valid_eq; eauto; now symmetry.
-Qed.
-
-End equality.
-
-(** *** Shift *)
-Section shift.
-
-Variable lb k k' k'' : Level.t.
-Variable t : t.
-
-Lemma shift_zero_refl : eq (shift lb 0 t) t.
+Lemma shift_zero_refl : eq (shift m 0 t) t.
 Proof. 
   destruct t; split; unfold RelationPairs.RelCompFun; simpl;
   try (apply O1.shift_zero_refl); now apply O2.shift_zero_refl.
 Qed.
 
-Lemma shift_trans : eq (shift lb k (shift lb k' t)) (shift lb (k + k') t).
+Lemma shift_trans : eq (shift m n (shift m k t)) (shift m (n + k) t).
 Proof. 
   destruct t; split; unfold RelationPairs.RelCompFun; simpl;
   try (apply O1.shift_trans); now apply O2.shift_trans.
 Qed.
 
-Lemma shift_permute : eq (shift lb k (shift lb k' t)) (shift lb k' (shift lb k t)).
+Lemma shift_permute : eq (shift m n (shift m k t)) (shift m k (shift m n t)).
 Proof. 
   destruct t; split; unfold RelationPairs.RelCompFun; simpl;
   try (apply O1.shift_permute); now apply O2.shift_permute.
 Qed.
 
-Lemma shift_unfold : eq (shift lb (k + k') t) (shift (lb + k) k' (shift lb k t)). 
+Lemma shift_unfold : eq (shift m (n + k) t) (shift (m + n) k (shift m n t)). 
 Proof. 
   destruct t; split; unfold RelationPairs.RelCompFun; simpl;
   try (apply O1.shift_unfold); now apply O2.shift_unfold.
 Qed.
 
 Lemma shift_unfold_1 :
-  k <= k' -> k' <= k'' -> 
-  eq (shift k' (k'' - k') (shift k  (k' - k) t)) (shift k (k'' - k) t).
+  n <= k -> k <= p -> 
+  eq (shift k (p - k) (shift n  (k - n) t)) (shift n (p - n) t).
 Proof.
   intros Hlt Hlt'; destruct t; unfold eq,shift; simpl; split; 
   unfold RelationPairs.RelCompFun; simpl.
@@ -114,65 +96,74 @@ Qed.
 
 End shift.
 
-(** *** Valid *)
-Section valid.
+(** **** [Wf] properties *)
 
-Lemma valid_weakening : forall k k' (t : t), 
-  (k <= k') -> valid k t -> valid k' t.
+#[export] Instance Wf_iff : Proper (Logic.eq ==> eq ==> iff) Wf.
 Proof.
-  intros. destruct H0,t0; split; simpl in *;
-  try (eapply O1.valid_weakening; eauto); 
-  eapply O2.valid_weakening; eauto.
+  repeat red; intros; subst; destruct x0,y0,H0.
+  unfold RelationPairs.RelCompFun in *; simpl in *.
+  split; intros; destruct H1; split; simpl in *;
+  try (eapply O1.Wf_iff; eauto; now symmetry);
+  eapply O2.Wf_iff; eauto; now symmetry.
 Qed.
 
-Lemma shift_preserves_valid : forall k k' t, 
-  valid k t -> valid (k + k') (shift k k' t).
+Lemma Wf_weakening (n k: Lvl.t) (t: t) : 
+  (n <= k) -> Wf n t -> Wf k t.
 Proof.
-  intros; destruct t0,H; split; simpl in *.
-  - now apply O1.shift_preserves_valid.
-  - now apply O2.shift_preserves_valid.
+  intros Hle Hvt. 
+  destruct Hvt,t; split; simpl in *;
+  try (eapply O1.Wf_weakening; eauto); 
+  eapply O2.Wf_weakening; eauto.
 Qed.
 
-Lemma shift_preserves_valid_1 : forall lb k k' t, 
-  valid k t -> valid (k + k') (shift lb k' t).
+Lemma shift_preserves_wf (n k: Lvl.t) (t: t) : 
+  Wf n t -> Wf (n + k) (shift n k t).
 Proof.
-  intros; destruct t0,H; split; simpl in *.
-  - now apply O1.shift_preserves_valid_1.
-  - now apply O2.shift_preserves_valid_1.
+  intros; destruct t,H; split; simpl in *.
+  - now apply O1.shift_preserves_wf.
+  - now apply O2.shift_preserves_wf.
 Qed.
 
-Lemma shift_preserves_valid_gen : forall lb lb' k k' t,  
-  k <= k' -> lb <= lb' -> k <= lb -> k' <= lb' ->
-  k' - k = lb' - lb ->  valid lb t -> valid lb' (shift k (k' - k) t).
+Lemma shift_preserves_wf_1 (m n k: Lvl.t) (t: t) : 
+  Wf n t -> Wf (n + k) (shift m k t).
 Proof.
-  intros; destruct t0,H4; split; simpl in *.
-  - now apply O1.shift_preserves_valid_gen with lb.
-  - now apply O2.shift_preserves_valid_gen with lb.
+  intros; destruct t,H; split; simpl in *.
+  - now apply O1.shift_preserves_wf_1.
+  - now apply O2.shift_preserves_wf_1.
 Qed.
 
-Lemma shift_preserves_valid_2 : forall lb lb' t, 
-  lb <= lb' -> valid lb t -> valid lb' (shift lb (lb' - lb) t).
-Proof.  intros. eapply shift_preserves_valid_gen; eauto. Qed.
+Lemma shift_preserves_wf_gen (m m' n k: Lvl.t) (t: t) :  
+  n <= k -> m <= m' -> n <= m -> k <= m' ->
+  k - n = m' - m ->  Wf m t -> Wf m' (shift n (k - n) t).
+Proof.
+  intros; destruct t,H4; split; simpl in *.
+  - now apply O1.shift_preserves_wf_gen with m.
+  - now apply O2.shift_preserves_wf_gen with m.
+Qed.
 
-Lemma shift_preserves_valid_zero : forall k t,
-  valid k t -> valid k (shift k 0 t).
+Lemma shift_preserves_wf_2 (m m': Lvl.t) (t: t) : 
+  m <= m' -> Wf m t -> Wf m' (shift m (m' - m) t).
+Proof.  intros. eapply shift_preserves_wf_gen; eauto. Qed.
+
+Lemma shift_preserves_wf_zero (n: Lvl.t) (t: t) :
+  Wf n t -> Wf n (shift n 0 t).
 Proof. 
-  intros; replace k with (k + 0); try lia; 
-  now apply shift_preserves_valid_1.
+  intros; replace n with (n + 0); try lia; 
+  now apply shift_preserves_wf_1.
 Qed.
-
-End valid.
 
 End IsLvlPairET.
 
 
+(** ---- *)
 
-(** ** Pair implementation with minimal constraints *)
+
+(** ** Leveled Pair Implementation - [ET] and [WL] *)
 Module IsLvlPairETWL (O1 : IsLvlETWL) (O2 : IsLvlETWL) <: IsLvlETWL.
 
 Include IsLvlPairET O1 O2.
 
-Lemma eq_leibniz : forall x y, eq x y -> x = y.
+Lemma eq_leibniz (x y: t) : eq x y -> x = y.
 Proof. 
   intros; destruct x,y; inversion H;
   unfold RelationPairs.RelCompFun in *; simpl in *.
@@ -182,66 +173,61 @@ Qed.
 
 End IsLvlPairETWL.
 
-(** ** Pair implementation with minimal constraints with [validb] *)
-Module IsLvlFullPairET (O1 : IsLvlFullET) 
-                                       (O2 : IsLvlFullET) 
-                                                <: IsLvlFullET.
 
-  Include IsLvlPairET O1 O2.
+(** ---- *)
 
-  (** *** Definition *)
-  Section definition.
 
-    Definition validb (lb : Level.t) (t : t) := 
-      (O1.validb lb (fst t)) && ((O2.validb lb) (snd t)).
+(** ** Leveled Pair Implementation - [ET] and [FL] *)
+Module IsLvlFullPairET (O1 : IsLvlFullET) (O2 : IsLvlFullET) <: IsLvlFullET.
 
-  End definition.
+Include IsLvlPairET O1 O2.
 
-  (** *** Equality *)
-  Section equality.
+(** *** Definition *)
+Definition is_wf (m : Lvl.t) (t : t) :=  (O1.is_wf m (fst t)) && ((O2.is_wf m) (snd t)).
 
-    Lemma validb_eq : Proper (Logic.eq ==> eq ==> Logic.eq) validb.
-    Proof.
-      repeat red; intros; destruct x0,y0,H0;
-      unfold RelationPairs.RelCompFun,validb in *; simpl in *; f_equal.
-      - eapply O1.validb_eq; eauto.
-      - eapply O2.validb_eq; eauto.
-    Qed.
+(** *** Properties *)
+Section is_wf.
 
-  End equality.
+Variable n : Lvl.t.
+Variable t : t.
 
-  (** *** Valid *)
-  Section valid.
+#[export] Instance is_wf_eq : Proper (Logic.eq ==> eq ==> Logic.eq) is_wf.
+Proof.
+  repeat red; intros; destruct x0,y0,H0;
+  unfold RelationPairs.RelCompFun,is_wf in *; simpl in *; f_equal.
+  - eapply O1.is_wf_eq; eauto.
+  - eapply O2.is_wf_eq; eauto.
+Qed.
 
-    Variable k : Level.t.
-    Variable t : t.
+Lemma Wf_is_wf_true : Wf n t <-> is_wf n t = true.
+Proof. 
+  destruct t; split; unfold is_wf,Wf; simpl;
+  rewrite andb_true_iff; intros [H1 H2]; split;
+  try (eapply O1.Wf_is_wf_true; eauto);
+  eapply O2.Wf_is_wf_true; eauto.
+Qed.
 
-    Lemma validb_valid : validb k t = true <-> valid k t.
-    Proof. 
-      destruct t; split; unfold validb,valid; simpl;
-      rewrite andb_true_iff; intros [H1 H2]; split;
-      try (eapply O1.validb_valid; eauto);
-      eapply O2.validb_valid; eauto.
-    Qed.
+Lemma notWf_is_wf_false : ~ Wf n t <-> is_wf n t = false.
+Proof.
+  intros; rewrite <- not_true_iff_false; split; intros; intro.
+  - apply H; now rewrite Wf_is_wf_true. 
+  - apply H; now rewrite <- Wf_is_wf_true.
+Qed. 
 
-    Lemma validb_nvalid : validb k t = false <-> ~ valid k t.
-    Proof.
-      intros; rewrite <- not_true_iff_false; split; intros; intro.
-      - apply H; now rewrite validb_valid. 
-      - apply H; now rewrite <- validb_valid.
-    Qed. 
-
-  End valid.
+End is_wf.
   
 End IsLvlFullPairET.
 
-(** ** Pair implementation with minimal constraints *)
-Module IsLvlFullPairETWL (O1 : IsLvlFullETWL) 
-                                   (O2 : IsLvlFullETWL) <: IsLvlFullETWL.
+
+(** ---- *)
+
+
+(** ** Leveled Pair Implementation - [ET], [WL] and [FL] *)
+Module IsLvlFullPairETWL (O1 : IsLvlFullETWL) (O2 : IsLvlFullETWL) <: IsLvlFullETWL.
 
 Include IsLvlFullPairET O1 O2.
 
-Lemma eq_leibniz : forall x y, eq x y -> x = y.
+Lemma eq_leibniz (x y: t) : eq x y -> x = y.
 Proof. 
   intros; destruct x,y; inversion H;
   unfold RelationPairs.RelCompFun in *; simpl in *.
@@ -251,28 +237,34 @@ Qed.
 
 End IsLvlFullPairETWL.
 
-(** ** Pair implementation with fully constrained *)
-Module IsBdlLvlPairET (O1 : IsBdlLvlET) 
-                                         (O2 : IsBdlLvlET) 
-                                                <: IsBdlLvlET.
 
-  Include IsLvlPairET O1 O2.
+(** ---- *)
 
-  Lemma shift_valid_refl : forall lb k t, valid lb t -> eq (shift lb k t) t.
-  Proof.
-    intros; destruct t0,H; split; unfold RelationPairs.RelCompFun;
-    simpl in *; try (now apply O1.shift_valid_refl);
-    now apply O2.shift_valid_refl.
-  Qed.
+
+(** ** Leveled Pair Implementation - [ET] and [BD] *)
+Module IsBdlLvlPairET (O1 : IsBdlLvlET) (O2 : IsBdlLvlET) <: IsBdlLvlET.
+
+Include IsLvlPairET O1 O2.
+
+Lemma shift_wf_refl (m n: Lvl.t) (t: t) : Wf m t -> eq (shift m n t) t.
+Proof.
+  intros; destruct t,H; split; unfold RelationPairs.RelCompFun;
+  simpl in *; try (now apply O1.shift_wf_refl);
+  now apply O2.shift_wf_refl.
+Qed.
   
 End IsBdlLvlPairET.
 
-Module IsBdlLvlPairETWL (O1 : IsBdlLvlETWL) 
-                                   (O2 : IsBdlLvlETWL) <: IsBdlLvlETWL.
+
+(** ---- *)
+
+
+(** ** Leveled Pair Implementation - [ET], [WL] and [BD] *)
+Module IsBdlLvlPairETWL (O1 : IsBdlLvlETWL) (O2 : IsBdlLvlETWL) <: IsBdlLvlETWL.
 
 Include IsBdlLvlPairET O1 O2.
 
-Lemma eq_leibniz : forall x y, eq x y -> x = y.
+Lemma eq_leibniz (x y: t) : eq x y -> x = y.
 Proof. 
   intros; destruct x,y; inversion H;
   unfold RelationPairs.RelCompFun in *; simpl in *.
@@ -282,29 +274,34 @@ Qed.
 
 End IsBdlLvlPairETWL.
 
-(** ** Pair implementation with fully constrained with [validb] *)
-Module IsBdlLvlFullPairET (O1 : IsBdlLvlFullET) 
-                                             (O2 : IsBdlLvlFullET) 
-                                                    <: IsBdlLvlFullET.
 
-  Include IsLvlFullPairET O1 O2.
+(** ---- *)
 
-  Lemma shift_valid_refl : forall lb k t, valid lb t -> eq (shift lb k t) t.
-  Proof.
-    intros; destruct t0,H; split; unfold RelationPairs.RelCompFun;
-    simpl in *; try (now apply O1.shift_valid_refl);
-    now apply O2.shift_valid_refl.
-  Qed.
-  
+
+(** ** Leveled Pair Implementation - [ET], [FL] and [BD] *)
+Module IsBdlLvlFullPairET (O1 : IsBdlLvlFullET) (O2 : IsBdlLvlFullET) <: IsBdlLvlFullET.
+
+Include IsLvlFullPairET O1 O2.
+
+Lemma shift_wf_refl (m n: Lvl.t) (t: t) : Wf m t -> eq (shift m n t) t.
+Proof.
+  intros; destruct t,H; split; unfold RelationPairs.RelCompFun;
+  simpl in *; try (now apply O1.shift_wf_refl);
+  now apply O2.shift_wf_refl.
+Qed.
+
 End IsBdlLvlFullPairET.
 
 
-Module IsBdlLvlFullPairETWL (O1 : IsBdlLvlFullETWL) 
-                                   (O2 : IsBdlLvlFullETWL) <: IsBdlLvlFullETWL.
+(** ---- *)
+
+
+(** ** Leveled Pair Implementation - [ET], [FL], [WL] and [BD] *)
+Module IsBdlLvlFullPairETWL (O1 : IsBdlLvlFullETWL) (O2 : IsBdlLvlFullETWL) <: IsBdlLvlFullETWL.
 
 Include IsBdlLvlFullPairET O1 O2.
 
-Lemma eq_leibniz : forall x y, eq x y -> x = y.
+Lemma eq_leibniz (x y: t) : eq x y -> x = y.
 Proof. 
   intros; destruct x,y; inversion H;
   unfold RelationPairs.RelCompFun in *; simpl in *.
@@ -315,36 +312,41 @@ Qed.
 End IsBdlLvlFullPairETWL.
 
 
-Module IsLvlPairOT (O1 : IsLvlOT) 
-                                   (O2 : IsLvlOT) <: IsLvlOT.
+(** ---- *)
+
+
+(** ** Leveled Pair Implementation - [OT] *)
+Module IsLvlPairOT (O1 : IsLvlOT) (O2 : IsLvlOT) <: IsLvlOT.
 
 Include OrdersEx.PairOrderedType O1 O2.
 
-(** *** Definition *)
-Section definition.
+(** *** Definitions *)
 
-Definition shift (lb k : Level.t) (t : t) := 
-  (O1.shift lb k (fst t),O2.shift lb k (snd t)).
+Definition shift (m n : Lvl.t) (t : t) := 
+  (O1.shift m n (fst t),O2.shift m n (snd t)).
 
-Definition valid (lb : Level.t) (t : t) := 
-  (O1.valid lb (fst t)) /\ ((O2.valid lb) (snd t)).
+Definition Wf (m : Lvl.t) (t : t) := 
+  (O1.Wf m (fst t)) /\ ((O2.Wf m) (snd t)).
 
-End definition.
+(** *** Properties *)
 
-(** *** Equality *)
-Section equality.
+(** **** [shift] properties *)
+Section shift.
 
-Lemma shift_eq : Proper (Logic.eq ==> Logic.eq ==> eq ==> eq) shift.
+Variable m n k p : Lvl.t.
+Variable t t1 : t.
+
+#[export] Instance shift_eq : Proper (Logic.eq ==> Logic.eq ==> eq ==> eq) shift.
 Proof.
   repeat red; intros; subst; destruct x1,y1.
   destruct H1; unfold RelationPairs.RelCompFun in *; simpl in *;
   split; try (now apply O1.shift_eq); now apply O2.shift_eq.
 Qed.
 
-Lemma shift_eq_iff : forall lb k t t1, 
-  eq t t1 <-> eq (shift lb k t) (shift lb k t1).
+Lemma shift_eq_iff :
+  eq t t1 <-> eq (shift m n t) (shift m n t1).
 Proof.
-  split; intro Heq; destruct t0,t1,Heq; split;
+  split; intro Heq; destruct t,t1,Heq; split;
   unfold RelationPairs.RelCompFun in *; simpl in *.
   - now apply O1.shift_eq_iff.
   - now apply O2.shift_eq_iff.
@@ -352,50 +354,33 @@ Proof.
   - rewrite O2.shift_eq_iff; eauto.
 Qed.
 
-Lemma valid_eq : Proper (Logic.eq ==> eq ==> iff) valid.
-Proof.
-  repeat red; intros; subst; destruct x0,y0,H0.
-  unfold RelationPairs.RelCompFun in *; simpl in *.
-  split; intros; destruct H1; split; simpl in *;
-  try (eapply O1.valid_eq; eauto; now symmetry);
-  eapply O2.valid_eq; eauto; now symmetry.
-Qed.
-
-End equality.
-
-(** *** Shift *)
-Section shift.
-
-Variable lb k k' k'' : Level.t.
-Variable t : t.
-
-Lemma shift_zero_refl : eq (shift lb 0 t) t.
+Lemma shift_zero_refl : eq (shift m 0 t) t.
 Proof. 
   destruct t; split; unfold RelationPairs.RelCompFun; simpl;
   try (apply O1.shift_zero_refl); now apply O2.shift_zero_refl.
 Qed.
 
-Lemma shift_trans : eq (shift lb k (shift lb k' t)) (shift lb (k + k') t).
+Lemma shift_trans : eq (shift m n (shift m k t)) (shift m (n + k) t).
 Proof. 
   destruct t; split; unfold RelationPairs.RelCompFun; simpl;
   try (apply O1.shift_trans); now apply O2.shift_trans.
 Qed.
 
-Lemma shift_permute : eq (shift lb k (shift lb k' t)) (shift lb k' (shift lb k t)).
+Lemma shift_permute : eq (shift m n (shift m k t)) (shift m k (shift m n t)).
 Proof. 
   destruct t; split; unfold RelationPairs.RelCompFun; simpl;
   try (apply O1.shift_permute); now apply O2.shift_permute.
 Qed.
 
-Lemma shift_unfold : eq (shift lb (k + k') t) (shift (lb + k) k' (shift lb k t)). 
+Lemma shift_unfold : eq (shift m (n + k) t) (shift (m + n) k (shift m n t)). 
 Proof. 
   destruct t; split; unfold RelationPairs.RelCompFun; simpl;
   try (apply O1.shift_unfold); now apply O2.shift_unfold.
 Qed.
 
 Lemma shift_unfold_1 :
-  k <= k' -> k' <= k'' -> 
-  eq (shift k' (k'' - k') (shift k  (k' - k) t)) (shift k (k'' - k) t).
+  n <= k -> k <= p -> 
+  eq (shift k (p - k) (shift n  (k - n) t)) (shift n (p - n) t).
 Proof.
   intros Hlt Hlt'; destruct t; unfold eq,shift; simpl; split; 
   unfold RelationPairs.RelCompFun; simpl.
@@ -405,65 +390,73 @@ Qed.
 
 End shift.
 
-(** *** Valid *)
-Section valid.
+(** *** [Wf] properties *)
 
-Lemma valid_weakening : forall k k' (t : t), 
-  (k <= k') -> valid k t -> valid k' t.
+#[export] Instance Wf_iff : Proper (Logic.eq ==> eq ==> iff) Wf.
 Proof.
-  intros. destruct H0,t0; split; simpl in *;
-  try (eapply O1.valid_weakening; eauto); 
-  eapply O2.valid_weakening; eauto.
+  repeat red; intros; subst; destruct x0,y0,H0.
+  unfold RelationPairs.RelCompFun in *; simpl in *.
+  split; intros; destruct H1; split; simpl in *;
+  try (eapply O1.Wf_iff; eauto; now symmetry);
+  eapply O2.Wf_iff; eauto; now symmetry.
 Qed.
 
-Lemma shift_preserves_valid : forall k k' t, 
-  valid k t -> valid (k + k') (shift k k' t).
+Lemma Wf_weakening (n k: Lvl.t) (t: t) : 
+  (n <= k) -> Wf n t -> Wf k t.
 Proof.
-  intros; destruct t0,H; split; simpl in *.
-  - now apply O1.shift_preserves_valid.
-  - now apply O2.shift_preserves_valid.
+  intros. destruct H0,t; split; simpl in *;
+  try (eapply O1.Wf_weakening; eauto); 
+  eapply O2.Wf_weakening; eauto.
 Qed.
 
-Lemma shift_preserves_valid_1 : forall lb k k' t, 
-  valid k t -> valid (k + k') (shift lb k' t).
+Lemma shift_preserves_wf (n k: Lvl.t) (t: t) : 
+  Wf n t -> Wf (n + k) (shift n k t).
 Proof.
-  intros; destruct t0,H; split; simpl in *.
-  - now apply O1.shift_preserves_valid_1.
-  - now apply O2.shift_preserves_valid_1.
+  intros; destruct t,H; split; simpl in *.
+  - now apply O1.shift_preserves_wf.
+  - now apply O2.shift_preserves_wf.
 Qed.
 
-Lemma shift_preserves_valid_gen : forall lb lb' k k' t,  
-  k <= k' -> lb <= lb' -> k <= lb -> k' <= lb' ->
-  k' - k = lb' - lb ->  valid lb t -> valid lb' (shift k (k' - k) t).
+Lemma shift_preserves_wf_1 (m n k: Lvl.t) (t: t) : 
+  Wf n t -> Wf (n + k) (shift m k t).
 Proof.
-  intros; destruct t0,H4; split; simpl in *.
-  - now apply O1.shift_preserves_valid_gen with lb.
-  - now apply O2.shift_preserves_valid_gen with lb.
+  intros; destruct t,H; split; simpl in *.
+  - now apply O1.shift_preserves_wf_1.
+  - now apply O2.shift_preserves_wf_1.
 Qed.
 
-Lemma shift_preserves_valid_2 : forall lb lb' t, 
-  lb <= lb' -> valid lb t -> valid lb' (shift lb (lb' - lb) t).
-Proof.  intros. eapply shift_preserves_valid_gen; eauto. Qed.
+Lemma shift_preserves_wf_gen (m m' n k: Lvl.t) (t: t) :  
+  n <= k -> m <= m' -> n <= m -> k <= m' ->
+  k - n = m' - m ->  Wf m t -> Wf m' (shift n (k - n) t).
+Proof.
+  intros; destruct t,H4; split; simpl in *.
+  - now apply O1.shift_preserves_wf_gen with m.
+  - now apply O2.shift_preserves_wf_gen with m.
+Qed.
 
-Lemma shift_preserves_valid_zero : forall k t,
-  valid k t -> valid k (shift k 0 t).
+Lemma shift_preserves_wf_2 (m m': Lvl.t) (t: t) : 
+  m <= m' -> Wf m t -> Wf m' (shift m (m' - m) t).
+Proof.  intros. eapply shift_preserves_wf_gen; eauto. Qed.
+
+Lemma shift_preserves_wf_zero (n: Lvl.t) (t: t) :
+  Wf n t -> Wf n (shift n 0 t).
 Proof. 
-  intros; replace k with (k + 0); try lia; 
-  now apply shift_preserves_valid_1.
+  intros; replace n with (n + 0); try lia; 
+  now apply shift_preserves_wf_1.
 Qed.
-
-End valid.
 
 End IsLvlPairOT.
 
 
-(** ** Pair implementation with minimal constraints *)
-Module IsLvlPairOTWL (O1 : IsLvlOTWL) 
-                                   (O2 : IsLvlOTWL) <: IsLvlOTWL.
+(** ---- *)
+
+
+(** ** Leveled Pair Implementation - [OT] and [WL] *)
+Module IsLvlPairOTWL (O1 : IsLvlOTWL) (O2 : IsLvlOTWL) <: IsLvlOTWL.
 
 Include IsLvlPairOT O1 O2.
 
-Lemma eq_leibniz : forall x y, eq x y -> x = y.
+Lemma eq_leibniz (x y: t) : eq x y -> x = y.
 Proof. 
   intros; destruct x,y; inversion H;
   unfold RelationPairs.RelCompFun in *; simpl in *.
@@ -473,65 +466,63 @@ Qed.
 
 End IsLvlPairOTWL.
 
-(** ** Pair implementation with minimal constraints with [validb] *)
-Module IsLvlFullPairOT (O1 : IsLvlFullOT) 
-                                       (O2 : IsLvlFullOT) 
-                                                <: IsLvlFullOT.
 
-  Include IsLvlPairOT O1 O2.
+(** ---- *)
 
-  (** *** Definition *)
-  Section definition.
 
-    Definition validb (lb : Level.t) (t : t) := 
-      (O1.validb lb (fst t)) && ((O2.validb lb) (snd t)).
+(** ** Leveled Pair Implementation - [OT] and [FL] *)
+Module IsLvlFullPairOT (O1 : IsLvlFullOT) (O2 : IsLvlFullOT) <: IsLvlFullOT.
 
-  End definition.
+Include IsLvlPairOT O1 O2.
 
-  (** *** Equality *)
-  Section equality.
+(** *** Definitions *)
 
-    Lemma validb_eq : Proper (Logic.eq ==> eq ==> Logic.eq) validb.
-    Proof.
-      repeat red; intros; destruct x0,y0,H0;
-      unfold RelationPairs.RelCompFun,validb in *; simpl in *; f_equal.
-      - eapply O1.validb_eq; eauto.
-      - eapply O2.validb_eq; eauto.
-    Qed.
+Definition is_wf (m : Lvl.t) (t : t) := 
+  (O1.is_wf m (fst t)) && ((O2.is_wf m) (snd t)).
 
-  End equality.
+(** *** Properties *)
+Section is_wf.
 
-  (** *** Valid *)
-  Section valid.
+Variable n : Lvl.t.
+Variable t : t.
 
-    Variable k : Level.t.
-    Variable t : t.
+Lemma is_wf_eq : Proper (Logic.eq ==> eq ==> Logic.eq) is_wf.
+Proof.
+  repeat red; intros; destruct x0,y0,H0;
+  unfold RelationPairs.RelCompFun,is_wf in *; simpl in *; f_equal.
+  - eapply O1.is_wf_eq; eauto.
+  - eapply O2.is_wf_eq; eauto.
+Qed.
 
-    Lemma validb_valid : validb k t = true <-> valid k t.
-    Proof. 
-      destruct t; split; unfold validb,valid; simpl;
-      rewrite andb_true_iff; intros [H1 H2]; split;
-      try (eapply O1.validb_valid; eauto);
-      eapply O2.validb_valid; eauto.
-    Qed.
+Lemma Wf_is_wf_true : Wf n t <-> is_wf n t = true.
+Proof. 
+  destruct t; split; unfold is_wf,Wf; simpl;
+  rewrite andb_true_iff; intros [H1 H2]; split;
+  try (eapply O1.Wf_is_wf_true; eauto);
+  eapply O2.Wf_is_wf_true; eauto.
+Qed.
 
-    Lemma validb_nvalid : validb k t = false <-> ~ valid k t.
-    Proof.
-      intros; rewrite <- not_true_iff_false; split; intros; intro.
-      - apply H; now rewrite validb_valid. 
-      - apply H; now rewrite <- validb_valid.
-    Qed. 
+Lemma notWf_is_wf_false : ~ Wf n t <-> is_wf n t = false.
+Proof.
+  intros; rewrite <- not_true_iff_false; split; intros; intro.
+  - apply H; now rewrite Wf_is_wf_true. 
+  - apply H; now rewrite <- Wf_is_wf_true.
+Qed. 
 
-  End valid.
+End is_wf.
   
 End IsLvlFullPairOT.
 
-Module IsLvlFullPairOTWL (O1 : IsLvlFullOTWL) 
-                                   (O2 : IsLvlFullOTWL) <: IsLvlFullOTWL.
+
+(** ---- *)
+
+
+(** ** Leveled Pair Implementation - [OT], [WL] and [FL] *)
+Module IsLvlFullPairOTWL (O1 : IsLvlFullOTWL) (O2 : IsLvlFullOTWL) <: IsLvlFullOTWL.
 
 Include IsLvlFullPairOT O1 O2.
 
-Lemma eq_leibniz : forall x y, eq x y -> x = y.
+Lemma eq_leibniz (x y: t) : eq x y -> x = y.
 Proof. 
   intros; destruct x,y; inversion H;
   unfold RelationPairs.RelCompFun in *; simpl in *.
@@ -541,28 +532,34 @@ Qed.
 
 End IsLvlFullPairOTWL.
 
-(** ** Pair implementation with fully constrained *)
-Module IsBdlLvlPairOT (O1 : IsBdlLvlOT) 
-                                         (O2 : IsBdlLvlOT) 
-                                                <: IsBdlLvlOT.
 
-  Include IsLvlPairOT O1 O2.
+(** ---- *)
 
-  Lemma shift_valid_refl : forall lb k t, valid lb t -> eq (shift lb k t) t.
-  Proof.
-    intros; destruct t0,H; split; unfold RelationPairs.RelCompFun;
-    simpl in *; try (now apply O1.shift_valid_refl);
-    now apply O2.shift_valid_refl.
-  Qed.
-  
+
+(** ** Leveled Pair Implementation - [OT] and [BD] *)
+Module IsBdlLvlPairOT (O1 : IsBdlLvlOT) (O2 : IsBdlLvlOT) <: IsBdlLvlOT.
+
+Include IsLvlPairOT O1 O2.
+
+Lemma shift_wf_refl (m n: Lvl.t) (t: t) : Wf m t -> eq (shift m n t) t.
+Proof.
+  intros; destruct t,H; split; unfold RelationPairs.RelCompFun;
+  simpl in *; try (now apply O1.shift_wf_refl);
+  now apply O2.shift_wf_refl.
+Qed.
+
 End IsBdlLvlPairOT.
 
-Module IsBdlLvlPairOTWL (O1 : IsBdlLvlOTWL) 
-                                   (O2 : IsBdlLvlOTWL) <: IsBdlLvlOTWL.
+
+(** ---- *)
+
+
+(** ** Leveled Pair Implementation - [OT], [WL] and [BD] *)
+Module IsBdlLvlPairOTWL (O1 : IsBdlLvlOTWL) (O2 : IsBdlLvlOTWL) <: IsBdlLvlOTWL.
 
 Include IsBdlLvlPairOT O1 O2.
 
-Lemma eq_leibniz : forall x y, eq x y -> x = y.
+Lemma eq_leibniz (x y: t) : eq x y -> x = y.
 Proof. 
   intros; destruct x,y; inversion H;
   unfold RelationPairs.RelCompFun in *; simpl in *.
@@ -572,28 +569,36 @@ Qed.
 
 End IsBdlLvlPairOTWL.
 
-(** ** Pair implementation with fully constrained with [validb] *)
+
+(** ---- *)
+
+
+(** ** Leveled Pair Implementation - [OT], [FL] and [BD] *)
 Module IsBdlLvlFullPairOT (O1 : IsBdlLvlFullOT) 
-                                             (O2 : IsBdlLvlFullOT) 
-                                                    <: IsBdlLvlFullOT.
+                           (O2 : IsBdlLvlFullOT) <: IsBdlLvlFullOT.
 
-  Include IsLvlFullPairOT O1 O2.
+Include IsLvlFullPairOT O1 O2.
 
-  Lemma shift_valid_refl : forall lb k t, valid lb t -> eq (shift lb k t) t.
-  Proof.
-    intros; destruct t0,H; split; unfold RelationPairs.RelCompFun;
-    simpl in *; try (now apply O1.shift_valid_refl);
-    now apply O2.shift_valid_refl.
-  Qed.
+Lemma shift_wf_refl (m n: Lvl.t) (t: t) : Wf m t -> eq (shift m n t) t.
+Proof.
+  intros; destruct t,H; split; unfold RelationPairs.RelCompFun;
+  simpl in *; try (now apply O1.shift_wf_refl);
+  now apply O2.shift_wf_refl.
+Qed.
   
 End IsBdlLvlFullPairOT.
 
+
+(** ---- *)
+
+
+(** ** Leveled Pair Implementation - [OT], [WL], [FL] and [BD] *)
 Module IsBdlLvlFullPairOTWL (O1 : IsBdlLvlFullOTWL) 
-                                   (O2 : IsBdlLvlFullOTWL) <: IsBdlLvlFullOTWL.
+                            (O2 : IsBdlLvlFullOTWL) <: IsBdlLvlFullOTWL.
 
 Include IsBdlLvlFullPairOT O1 O2.
 
-Lemma eq_leibniz : forall x y, eq x y -> x = y.
+Lemma eq_leibniz (x y: t) : eq x y -> x = y.
 Proof. 
   intros; destruct x,y; inversion H;
   unfold RelationPairs.RelCompFun in *; simpl in *.
