theories/Set/Levels.v
@@ -1,42 +1,178 @@
 From Coq Require Import MSets Lia.
-From DeBrLevel Require Import LevelInterface Level SetLevelInterface SetLevel.
+From DeBrLevel Require Import LevelInterface Level SetLevelInterface SetLevel SetOTwL SetOTwLInterface.
 
-(** * Implementation - Level Set
+(** * Implementation - Set of levels
 
-  A level set has extra permutation property because of elements of the set can
-  interact with [shift] parameters.
+  A level set has extra permutation properties because of elements of the set can
+  interact with [shift] parameters. We also define [new_key] function as done for maps.
 *)
-Module Levels <: IsBdlLvlFullOTWL.
+Module Levels (Import Se : SetOTWithLeibnizInterface Level) <: IsLvlSetLVLInterface Se.
 
-Include MakeBdlLvlFullSet Level.
-Import St.
+Include IsBdlLvlFullSet Level Se.
 
-Lemma shift_permute_1 : forall (t : t) lb k k',
-  eq (shift lb k (shift lb k' t)) (shift (lb + k) k' (shift lb k t)).
+(** *** Definitions *)
+
+Definition max_key (s: t) := fold (Nat.max) s 0.
+Definition new_key (s: t) := if is_empty s then 0 else S (max_key s).
+
+(** *** Properties *)
+
+(** **** [max_key] properties *)
+
+#[export] Instance max_eq : Proper (Logic.eq ==> Logic.eq ==> Logic.eq) max := _.
+#[export] Instance logic_eq : Equivalence Logic.eq := _.
+
+Lemma max_transpose : transpose Logic.eq max.
 Proof.
-  intro t; induction t using set_induction; intros.
-  - repeat rewrite shift_Empty_spec; eauto. reflexivity.
-  - apply Add_inv in H0; subst. repeat rewrite shift_add_notin_spec; auto.
+ intros x y z; lia.
+Qed.
+
+#[export] Hint Resolve max_eq max_transpose logic_eq : core.
+
+#[export] Instance max_key_eq : Proper (eq ==> Logic.eq) max_key.
+Proof.
+  intros s s' Heq.
+  apply eq_leibniz in Heq; now subst.
+Qed. 
+
+Lemma max_key_Empty (s: t) : Empty s -> max_key s = 0.
+Proof.
+  unfold max_key; intro HEmp.
+  apply empty_is_empty_1 in HEmp.
+  apply eq_leibniz in HEmp; subst.
+  now rewrite fold_empty.
+Qed.
+
+Lemma max_key_empty : max_key empty = 0.
+Proof. unfold max_key; now rewrite fold_empty. Qed.
+
+Lemma max_key_add_max (v: elt) (s: t) : max_key (add v s) = max v (max_key s).
+Proof.
+  unfold max_key.
+  destruct (In_dec v s).
+  - assert (s = add v (remove v s)).
+    -- apply eq_leibniz.
+       rewrite add_remove; auto; reflexivity.
+    -- assert (s = add v s).
+       + apply eq_leibniz.
+         rewrite add_equal; auto; reflexivity.
+       + rewrite <- H0.
+         rewrite H.
+         rewrite fold_add; auto; try lia.
+         rewrite remove_spec; intros [HIn Hc]; contradiction.
+  - rewrite fold_add; auto.
+Qed.
+
+Lemma max_key_Add_max (v: elt) (s s': t) : Add v s s' -> max_key s' = max v (max_key s).
+Proof.
+  intro HA.
+  apply Add_inv in HA; subst.
+  apply max_key_add_max.
+Qed.
+
+(** **** [new_key] properties *)
+
+#[export] Instance new_key_eq : Proper (eq ==> Logic.eq) new_key.
+Proof.
+  intros s s' Heq; unfold new_key.
+  rewrite Heq.
+  erewrite max_key_eq; eauto. 
+Qed.
+
+Lemma new_key_Empty (s: t) : Empty s -> new_key s = 0.
+Proof.
+  unfold new_key; intro HEmp.
+  rewrite <- is_empty_spec in HEmp.
+  now rewrite HEmp.
+Qed.
+
+Lemma new_key_empty : new_key empty = 0.
+Proof.
+  apply new_key_Empty.
+  apply empty_spec.
+Qed.
+
+Lemma new_key_add_max (v: elt) (s: t) : new_key (add v s) = max (S v) (new_key s).
+Proof.
+  unfold new_key.
+  destruct (is_empty s) eqn:Hemp.
+  - destruct (is_empty (add v s)) eqn:Hemp'.
+    -- apply is_empty_spec in Hemp'.
+       exfalso; apply (Hemp' v).
+       rewrite add_spec; auto.
+    -- rewrite max_key_add_max.
+       rewrite max_key_Empty.
+       + lia.
+       + now apply is_empty_spec.
+  - destruct (is_empty (add v s)) eqn:Hemp'.
+    -- apply is_empty_spec in Hemp'.
+       exfalso; apply (Hemp' v).
+       rewrite add_spec; auto.
+    -- rewrite max_key_add_max; lia.
+Qed.
+
+Lemma new_key_Add_max (v: elt) (s s': t) : Add v s s' -> new_key s' = max (S v) (new_key s).
+Proof.
+  intro HA.
+  apply Add_inv in HA; subst.
+  apply new_key_add_max.
+Qed.
+
+Lemma new_key_in_spec (v: elt) (s: t) : In v s -> (v < new_key s)%nat.
+Proof.
+  revert v.
+  induction s using set_induction; intros b HIn.
+  - exfalso.
+    apply (H b HIn).
+  - apply Add_inv in H0; subst.
+    apply add_spec in HIn as [Heq | HIn]; subst.
+    -- rewrite new_key_add_max; lia.
+    -- rewrite new_key_add_max.
+       apply IHs1 in HIn; lia.
+Qed.
+
+(** **** [shift] properties *)
+
+Lemma shift_permute_1 (m n k: Lvl.t) (s: t) :
+  eq (shift m n (shift m k s)) (shift (m + n) k (shift m n s)).
+Proof.
+  induction s using set_induction; intros.
+  - repeat rewrite shift_Empty; eauto. reflexivity.
+  - apply Add_inv in H0; subst. repeat rewrite shift_add_notin; auto.
     -- split; intros; rewrite add_spec in *; destruct H0;
         try (left; rewrite H0; now rewrite Level.shift_permute_1);
-        right; now rewrite IHt1 in *.
+        right; now rewrite IHs1 in *.
     -- rewrite shift_notin_iff in H; eauto.
     -- rewrite shift_notin_iff in H; eauto.
 Qed.
 
-Lemma shift_permute_2 : forall (t : t) lb lb' k k',
-  lb <= lb' -> eq (shift lb k (shift lb' k' t)) (shift (lb' + k) k' (shift lb k t)).
+Lemma shift_permute_2 (m n k p: Lvl.t) (s: t) :
+  m <= n -> eq (shift m k (shift n p s)) (shift (n + k) p (shift m k s)).
 Proof.
-  intro t. induction t using set_induction; intros.
-  - repeat rewrite shift_Empty_spec; eauto; reflexivity.
-  - apply Add_inv in H0; subst. repeat rewrite shift_add_notin_spec; auto.
+  induction s using set_induction; intros.
+  - repeat rewrite shift_Empty; eauto; reflexivity.
+  - apply Add_inv in H0; subst. repeat rewrite shift_add_notin; auto.
     -- split; intros; rewrite add_spec in *; destruct H0.
         + subst; left; now apply Level.shift_permute_2.
-        + right. rewrite IHt1 in H0; auto.
+        + right. rewrite IHs1 in H0; auto.
         + subst; left; symmetry; now apply Level.shift_permute_2.
-        + right. rewrite <- IHt1 in H0; auto.
+        + right. rewrite <- IHs1 in H0; auto.
     -- rewrite shift_notin_iff in H; eauto.
     -- rewrite shift_notin_iff in H; eauto.
 Qed.
 
 End Levels.
+
+
+(** ---- *)
+
+
+(** * Make - Set of levels *)
+
+Module MakeLVL <: IsBdlLvlFullOTWL.
+
+Module St := SetOTWithLeibniz Level.
+Include Levels St.
+Import St.
+
+End MakeLVL.
