theories/Set/SetLevel.v
@@ -1,14 +1,16 @@
 From Coq Require Import MSets Lia.
 From DeBrLevel Require Import Level LevelInterface SetLevelInterface SetOTwL SetOTwLInterface.
 
-(** * Implementation - Leveled Set *)
+(** * Implementation - Leveled Set 
 
-(** ** Leveled Map Implementation *)
-Module IsLvlSet 
-  (T : IsLvlOTWL) (Import St : SetOTWithLeibnizInterface T) <: IsLvlSetInterface T St.
+We use the notation [OT] when elements satisfy [Ordered Type] module, [WL] when the embedded type has an equivalent equality to the one from Coq, [FL] when the embbeded type has boolean version of [Wf] and finally [BD] when elements does not contains binders associated to levels.
+*)
+
+(** ** Leveled Set Implementation - [OT] and [WL] *)
+Module IsLvlSet (T : IsLvlOTWL) (Import St : SetOTWithLeibnizInterface T) <: IsLvlSetInterface T St.
 
 
-(** *** Definition *)
+(** *** Definitions *)
 
 Definition t := t.
 
@@ -24,96 +26,96 @@ Definition lt_compat := lt_compat.
 Definition compare := compare.
 Definition compare_spec := compare_spec.
 
-Definition shift (lb : nat) (k : nat) (s : t) : t := map (T.shift lb k) s.
+Definition shift (m k: Lvl.t) (s: t) : t := map (T.shift m k) s.
+Definition Wf (k: Lvl.t) (s: t) := (For_all (T.Wf k) s).
 
-Definition valid (k : nat) (s : t) := (For_all (T.valid k) s).
+(** *** Properties *)
 
-(** *** [valid] property *)
-Section valid.
+(** **** [Wf] properties *)
+Section specs.
 
-Variable lb : nat.
+Variable m n k : Lvl.t.
 Variable v : elt.
 Variable s s' : t.
 
-Lemma valid_unfold : valid lb s <-> (For_all (T.valid lb) s).
-Proof. unfold valid; split; auto. Qed.
 
-Lemma valid_add_spec : valid lb (add v s) -> T.valid lb v /\ valid lb s.
-Proof.
-  intros; unfold valid,For_all in *; split.
-  - apply H; apply add_spec; now left.
-  - intros. apply H; apply add_spec; now right.
-Qed.
-
-Lemma valid_empty_spec : valid lb empty.
-Proof. intros; unfold valid,For_all; intros; inversion H. Qed.
-
-Lemma valid_union_iff : valid lb (union s s') <-> valid lb s /\ valid lb s'.
-Proof.
-  split; intros; unfold valid,For_all in *.
-  - split; intros; apply H; rewrite union_spec; auto.
-  - intros; destruct H; rewrite union_spec in *; destruct H0; auto.
-Qed.
-
-Lemma valid_singleton_iff : valid lb (singleton v) <-> T.valid lb v.
-Proof.
-  split; intros; unfold valid,For_all in *.
-  - apply H; now rewrite singleton_spec.
-  - intros; rewrite singleton_spec in H0. apply T.eq_leibniz in H0; now subst.
-Qed.
-
-Lemma valid_in_spec : valid lb s -> In v s -> T.valid lb v.
-Proof.
-  unfold valid,For_all in *; intros; now apply H.
-Qed.
-
-#[export]
-Instance valid_eq : Proper (Logic.eq ==> eq ==> iff) valid.
+#[export] Instance Wf_iff : Proper (Logic.eq ==> eq ==> iff) Wf.
 Proof.
   repeat red; intros; apply eq_leibniz in H0; subst; split; auto.
 Qed.
 
-Lemma valid_weakening: forall k k' s,
-  (k <= k') -> valid k s -> valid k' s.
-Proof. 
-  intros; unfold valid,For_all in *; intros; apply H0 in H1. 
-  eapply T.valid_weakening; eauto.
+Lemma Wf_unfold : Wf m s <-> (For_all (T.Wf m) s).
+Proof. unfold Wf; split; auto. Qed.
+
+Lemma Wf_add_iff : Wf m (add v s) <-> T.Wf m v /\ Wf m s.
+Proof.
+  split.
+  - intros; unfold Wf,For_all in *; split.
+    -- apply H; apply add_spec; now left.
+    -- intros. apply H; apply add_spec; now right.
+  - intros [Hwfv HWfs].
+    unfold Wf, For_all in *.
+    intros x HIn.
+    apply add_spec in HIn as [Heq | HIn].
+    -- now apply T.eq_leibniz in Heq; subst.
+    -- now apply HWfs.
 Qed.
 
-End valid.
+Lemma Wf_empty : Wf m empty.
+Proof. intros; unfold Wf,For_all; intros; inversion H. Qed.
 
-(** *** [shift] property *)
-Section shift.
+Lemma Wf_union_iff : Wf m (union s s') <-> Wf m s /\ Wf m s'.
+Proof.
+  split; intros; unfold Wf,For_all in *.
+  - split; intros; apply H; rewrite union_spec; auto.
+  - intros; destruct H; rewrite union_spec in *; destruct H0; auto.
+Qed.
 
-Variable lb k : nat.
-Variable v : elt.
-Variable s : t.
+Lemma Wf_singleton_iff : Wf m (singleton v) <-> T.Wf m v.
+Proof.
+  split; intros; unfold Wf,For_all in *.
+  - apply H; now rewrite singleton_spec.
+  - intros; rewrite singleton_spec in H0. apply T.eq_leibniz in H0; now subst.
+Qed.
+
+Lemma Wf_in : Wf m s -> In v s -> T.Wf m v.
+Proof.
+  unfold Wf,For_all in *; intros; now apply H.
+Qed.
+
+Lemma Wf_weakening : (m <= n) -> Wf m s -> Wf n s.
+Proof. 
+  intros; unfold Wf,For_all in *; intros; apply H0 in H1. 
+  eapply T.Wf_weakening; eauto.
+Qed.
+
+(** **** [shift] properties *)
 
 #[local] Hint Resolve eq_equiv transpose_1 proper_1 : core.
 
-Lemma shift_union_spec : forall s', 
-  shift lb k (union s s') = union (shift lb k s) (shift lb k s').
+Lemma shift_union :
+  shift m k (union s s') = union (shift m k s) (shift m k s').
 Proof. intros; unfold shift; now rewrite map_union_spec. Qed.
 
-Lemma shift_Empty_spec : Empty s -> shift lb k s = empty.
+Lemma shift_Empty : Empty s -> shift m k s = empty.
 Proof. intros; unfold shift; now apply map_Empty_spec. Qed.
 
-Lemma shift_empty_spec : shift lb k empty = empty.
+Lemma shift_empty : shift m k empty = empty.
 Proof. intros; unfold shift; now apply map_empty_spec. Qed.
 
-Lemma shift_singleton_spec : shift lb k (singleton v) = singleton (T.shift lb k v).
+Lemma shift_singleton : shift m k (singleton v) = singleton (T.shift m k v).
 Proof. intros; unfold shift; now apply map_singleton_spec. Qed.
 
-Lemma shift_add_notin_spec :
-  ~ In v s -> shift lb k (add v s) = add (T.shift lb k v) (shift lb k s).
+Lemma shift_add_notin :
+  ~ In v s -> shift m k (add v s) = add (T.shift m k v) (shift m k s).
 Proof. intros; unfold shift; now apply map_add_notin_spec. Qed.
 
-Lemma shift_add_in_spec :
-  In v s -> shift lb k (add v s) = (shift lb k s).
+Lemma shift_add_in :
+  In v s -> shift m k (add v s) = (shift m k s).
 Proof. intros; unfold shift; now apply map_add_in_spec. Qed.
 
 Lemma shift_in_iff :
-  In v s <-> In (T.shift lb k v) (shift lb k s).
+  In v s <-> In (T.shift m k v) (shift m k s).
 Proof.
   unfold shift; induction s using set_induction.
   - split; intro HIn; rewrite map_Empty_spec in *; auto; apply empty_is_empty_1 in H; 
@@ -126,19 +128,19 @@ Proof.
     -- rewrite <- IHt0_1 in H0; now right.
 Qed.
 
-Lemma shift_add_spec :
-  shift lb k (add v s) = add (T.shift lb k v) (shift lb k s).
+Lemma shift_add :
+  shift m k (add v s) = add (T.shift m k v) (shift m k s).
 Proof.
   intros; destruct (In_dec v s).
-  - rewrite shift_add_in_spec; auto. apply eq_leibniz; rewrite add_equal.
+  - rewrite shift_add_in; auto. apply eq_leibniz; rewrite add_equal.
     -- reflexivity.
     -- now apply shift_in_iff.
-  - now  apply shift_add_notin_spec.
+  - now  apply shift_add_notin.
 Qed.
 
-Lemma shift_in_e_spec :
-  In v (shift lb k s) -> 
-  exists v', v = (T.shift lb k v') /\  In (T.shift lb k v') (shift lb k s).
+Lemma shift_in_e :
+  In v (shift m k s) -> 
+  exists v', v = (T.shift m k v') /\  In (T.shift m k v') (shift m k s).
 Proof.
   induction s using set_induction; intro HI; unfold shift in *.
   - rewrite map_Empty_spec in HI; auto; inversion HI.
@@ -150,70 +152,70 @@ Proof.
       exists r'; split; auto. rewrite map_add_notin_spec; auto; rewrite add_spec; now right.
 Qed. 
 
-Lemma shift_notin_iff : ~ In v s <-> ~ In (T.shift lb k v) (shift lb k s).
+Lemma shift_notin_iff : ~ In v s <-> ~ In (T.shift m k v) (shift m k s).
 Proof.
   intros; split; unfold not; intros; apply H.
   - now rewrite <- shift_in_iff in H0.
   - now rewrite <- shift_in_iff.
 Qed.
 
-End shift.
+End specs.
 
-Lemma shift_remove_spec : forall lb k v s,
-  shift lb k (remove v s) = remove (T.shift lb k v)(shift lb k s).
+Lemma shift_remove (m k: Lvl.t) (v: elt) (s: t) :
+  shift m k (remove v s) = remove (T.shift m k v)(shift m k s).
 Proof.
-  intros lb k v s; revert lb k v;
+  revert m k v;
   induction s using set_induction; intros.
-  - symmetry; rewrite shift_Empty_spec; auto. 
+  - symmetry; rewrite shift_Empty; auto. 
     apply empty_is_empty_1 in H. eapply Equal_remove in H; apply eq_leibniz in H; rewrite H.
     apply eq_leibniz. split; intros.
     -- rewrite remove_spec in H0; destruct H0. inversion H0.
-    -- apply shift_in_e_spec in H0.
+    -- apply shift_in_e in H0.
         destruct H0. destruct H0.
         apply shift_in_iff in H1. rewrite remove_spec in H1; destruct H1; inversion H1.
   
   - apply Add_inv in H0; subst. apply eq_leibniz; split; intros.
-    -- apply shift_in_e_spec in H0. destruct H0; destruct H0.
+    -- apply shift_in_e in H0. destruct H0; destruct H0.
         apply shift_in_iff in H1. apply remove_spec in H1 as [H1 H1'].
         rewrite remove_spec; split; subst.
         + now apply shift_in_iff.
         + intro; apply H1'. eapply T.shift_eq_iff; eauto.
-    -- apply remove_spec in H0 as [H0 H0']. rewrite shift_add_notin_spec in H0; auto.
+    -- apply remove_spec in H0 as [H0 H0']. rewrite shift_add_notin in H0; auto.
         apply add_spec in H0; destruct H0; subst.
         + apply T.eq_leibniz in H0; subst; apply shift_in_iff. apply remove_spec; split.
           ++ apply add_spec; now left.
           ++ intro; apply H0'; subst; auto; apply T.eq_leibniz in H0;
             subst; reflexivity.
-        + apply shift_in_e_spec in H0; destruct H0 as [y [Heq HIn]]; subst.
+        + apply shift_in_e in H0; destruct H0 as [y [Heq HIn]]; subst.
           apply shift_in_iff. rewrite remove_spec; split.
           ++ apply add_spec; right; now apply shift_in_iff in HIn.
           ++ intro; apply H0'; apply T.eq_leibniz in H0; now subst.
 Qed.
 
-Lemma shift_eq_iff : forall lb k s s',
-  eq s s' <-> eq (shift lb k s) (shift lb k s').
+Lemma shift_eq_iff (m k: Lvl.t) (s s': t) :
+  eq s s' <-> eq (shift m k s) (shift m k s').
 Proof.
   split.
   - intro Heq; apply eq_leibniz in Heq; now subst.
-  - revert lb k s'; induction s using set_induction; intros lb k s'' Heq.
+  - revert m k s'; induction s using set_induction; intros m k s'' Heq.
     -- apply empty_is_empty_1 in H as H'.
-        apply eq_leibniz in H'; subst. eapply shift_Empty_spec in H; rewrite H in *.
-        symmetry in Heq. clear H. symmetry. revert lb k Heq.
+        apply eq_leibniz in H'; subst. eapply shift_Empty in H; rewrite H in *.
+        symmetry in Heq. clear H. symmetry. revert m k Heq.
         induction s'' using set_induction; intros.
         * apply empty_is_empty_1 in H; now rewrite H.
-        * apply Add_inv in H0; subst. rewrite shift_add_notin_spec in Heq; auto.
+        * apply Add_inv in H0; subst. rewrite shift_add_notin in Heq; auto.
 
-          assert (eq (add (T.shift lb k x) (shift lb k s''1)) empty).
+          assert (eq (add (T.shift m k x) (shift m k s''1)) empty).
           { now rewrite Heq. }
 
           apply empty_is_empty_2 in H0; unfold Empty in H0; exfalso.
-          apply (H0 (T.shift lb k x)). rewrite add_spec; now left.
+          apply (H0 (T.shift m k x)). rewrite add_spec; now left.
     -- apply Add_inv in H0; subst.
 
         assert (forall s s' v, (add v s) = s' -> In v s').
         { intros; subst; apply add_spec; now left. }
 
-        rewrite shift_add_notin_spec in Heq; auto. apply eq_leibniz in Heq.
+        rewrite shift_add_notin in Heq; auto. apply eq_leibniz in Heq.
         apply H0 in Heq as Heq'. apply add_remove in Heq' as Htmp.
         apply eq_leibniz in Htmp. rewrite <- Htmp in Heq; clear Htmp.
         rewrite <- shift_in_iff in Heq'. apply add_remove in Heq' as Htmp.
@@ -224,16 +226,16 @@ Proof.
         
         apply H1; clear H1. f_equal. apply eq_leibniz; eapply IHs1.
         rewrite <- add_eq_leibniz in Heq; eauto.
-        * rewrite Heq. now rewrite shift_remove_spec.
+        * rewrite Heq. now rewrite shift_remove.
         * now apply shift_notin_iff.
         * rewrite remove_spec; intro. destruct H1; auto.
           apply H2; reflexivity.
 Qed.
 
-Lemma shift_inter_spec : forall lb k s s', 
-  shift lb k (inter s s') = inter (shift lb k s) (shift lb k s').
+Lemma shift_inter (m k: Lvl.t) (s s': t) : 
+  shift m k (inter s s') = inter (shift m k s) (shift m k s').
 Proof.
-  intros lb k s; induction s using set_induction; intros.
+  revert s'; induction s using set_induction; intros.
   - apply empty_inter_1 with (s' := s') in H as H'.
     unfold shift; rewrite map_Empty_spec; auto.
     symmetry; rewrite map_Empty_spec; auto. apply eq_leibniz; split; intros.
@@ -244,21 +246,21 @@ Proof.
     destruct (In_dec x s').
     -- rewrite inter_in_add_spec; auto. rewrite map_add_notin_spec.
       + symmetry; rewrite map_add_notin_spec; auto.
-        rewrite (shift_in_iff lb k) in i.
+        rewrite (shift_in_iff m k) in i.
         rewrite inter_in_add_spec; auto.
         unfold shift in *. now rewrite IHs1.
       + unfold not; intros; rewrite inter_spec in H0; destruct H0; contradiction.
 
     -- rewrite inter_notin_add_spec; auto. rewrite map_add_notin_spec; auto.
-      rewrite (shift_notin_iff lb k) in n.
+      rewrite (shift_notin_iff m k) in n.
       rewrite inter_notin_add_spec; auto.
       unfold shift in *. now rewrite IHs1.
 Qed.
 
-Lemma shift_diff_spec : forall lb k s s',
-  shift lb k (diff s s') = (diff (shift lb k s) (shift lb k s')).
+Lemma shift_diff (m k: Lvl.t) (s s': t) :
+  shift m k (diff s s') = (diff (shift m k s) (shift m k s')).
 Proof.
-  intros lb k s; induction s using set_induction; intros.
+  revert s'; induction s using set_induction; intros.
 
   - apply eq_leibniz; split; unfold shift; intros.
     -- apply empty_diff_1 with (s' := s') in H; rewrite map_Empty_spec in H0; auto.
@@ -276,8 +278,8 @@ Proof.
         rewrite map_add_notin_spec; auto; rewrite add_spec; auto.
 
       + rewrite diff_notin_add_spec in H1; auto. rewrite diff_spec in *.
-        replace (shift lb k (add x (diff s1 s')))
-        with ( add (T.shift lb k x) (shift lb k (diff s1 s'))) in H1.
+        replace (shift m k (add x (diff s1 s')))
+        with ( add (T.shift m k x) (shift m k (diff s1 s'))) in H1.
         ++ rewrite add_spec in H1; destruct H1.
             * rewrite H0; split.
               ** unfold shift; rewrite map_add_notin_spec; auto.
@@ -317,8 +319,8 @@ Proof.
             * apply diff_notin_spec; auto.
 Qed.
 
-Lemma shift_zero_refl : forall lb s,
-  eq (shift lb 0 s) s.
+Lemma shift_zero_refl (m: Lvl.t) (s: t) :
+  eq (shift m 0 s) s.
 Proof.
   unfold shift; intros. induction s using set_induction.
   - apply empty_is_empty_1 in H; apply eq_leibniz in H; subst.  
@@ -327,15 +329,16 @@ Proof.
     apply eq_leibniz in IHs1; rewrite IHs1; rewrite T.shift_zero_refl; reflexivity.
 Qed.
 
-Lemma shift_eq : Proper (Logic.eq ==> Logic.eq ==> eq ==> eq) shift.
+#[export] Instance shift_eq : Proper (Logic.eq ==> Logic.eq ==> eq ==> eq) shift.
 Proof. 
-  red; red; red; red; intros; subst. apply eq_leibniz in H1; now subst.
+  red; red; red; red; intros; subst. 
+  apply eq_leibniz in H1; now subst.
 Qed.
 
-Lemma shift_trans : forall lb k k' s,
-  eq (shift lb k (shift lb k' s)) (shift lb (k + k') s).
+Lemma shift_trans (m n k: Lvl.t) (s: t) :
+  eq (shift m n (shift m k s)) (shift m (n + k) s).
 Proof.
-  intros lb k k' s; induction s using set_induction; unfold shift.
+  induction s using set_induction; unfold shift.
   - repeat rewrite map_Empty_spec; auto; reflexivity.
   - apply Add_inv in H0; subst. repeat rewrite map_add_notin_spec; auto.
     -- split; intros HI; rewrite add_spec in *; destruct HI.
@@ -346,10 +349,10 @@ Proof.
     -- rewrite shift_notin_iff in H; eauto.
 Qed.
 
-Lemma shift_permute : forall lb k k' s,
-  eq (shift lb k (shift lb k' s)) (shift lb k' (shift lb k s)).
+Lemma shift_permute (m n k: Lvl.t) (s: t) :
+  eq (shift m n (shift m k s)) (shift m k (shift m n s)).
 Proof.
-  intros lb k k' s; induction s using set_induction; unfold shift.
+  induction s using set_induction; unfold shift.
   - repeat rewrite map_Empty_spec; auto; reflexivity.
   - apply Add_inv in H0; subst; repeat rewrite map_add_notin_spec; auto;
     try (rewrite shift_notin_iff in H; now eauto).
@@ -360,140 +363,181 @@ Proof.
     -- right; unfold shift in *; now rewrite IHs1.
 Qed.
 
-Lemma shift_unfold : forall lb k k' t,
-  eq (shift lb (k + k') t) (shift (lb + k) k' (shift lb k t)). 
+Lemma shift_unfold (m n k: Lvl.t) (t: t) :
+  eq (shift m (n + k) t) (shift (m + n) k (shift m n t)). 
 Proof.
-  intros lb k k' t; induction t using set_induction.
+  induction t using set_induction.
   - unfold shift; repeat rewrite map_Empty_spec; auto. reflexivity.
-  - apply Add_inv in H0; subst. repeat rewrite shift_add_notin_spec; eauto.
+  - apply Add_inv in H0; subst. repeat rewrite shift_add_notin; eauto.
     -- rewrite T.shift_unfold; rewrite IHt1; reflexivity.
     -- now apply shift_notin_iff.
 Qed.
 
-Lemma shift_unfold_1 : forall k k' k'' t,
-  k <= k' -> k' <= k'' -> 
-  eq (shift k' (k'' - k') (shift k  (k' - k) t)) (shift k (k'' - k) t).
+Lemma shift_unfold_1 (m n p: Lvl.t) (t: t) :
+  m <= n -> n <= p -> 
+  eq (shift n (p - n) (shift m  (n - m) t)) (shift m (p - m) t).
 Proof.
-  intros k k' k'' t; induction t using set_induction; intros.
+  induction t using set_induction; intros.
   - unfold shift; repeat rewrite map_Empty_spec; auto. reflexivity.
-  - apply Add_inv in H0; subst. repeat rewrite shift_add_notin_spec; eauto.
+  - apply Add_inv in H0; subst. repeat rewrite shift_add_notin; eauto.
     -- rewrite T.shift_unfold_1; auto; rewrite IHt1; auto; reflexivity.
     -- now apply shift_notin_iff.
 Qed.
 
-(** *** Interaction property between [valid] and [shift] *)
+(** **** Interaction properties between [Wf] and [shift] *)
 
-Theorem shift_preserves_valid_1 : forall lb k k' s,
-  valid k s -> valid (k + k') (shift lb k' s).
+Theorem shift_preserves_wf_1 (m n k: Lvl.t) (s: t) :
+  Wf n s -> Wf (n + k) (shift m k s).
 Proof.
-  unfold valid,For_all in *; intros.
-  apply shift_in_e_spec in H0; destruct H0 as [y [Heq HIn]]; subst.
-  apply T.shift_preserves_valid_1; apply H; now rewrite <- shift_in_iff in HIn.
+  unfold Wf,For_all in *; intros.
+  apply shift_in_e in H0; destruct H0 as [y [Heq HIn]]; subst.
+  apply T.shift_preserves_wf_1; apply H; now rewrite <- shift_in_iff in HIn.
 Qed.
 
-Theorem shift_preserves_valid : forall k k' s,
-  valid k s -> valid (k + k') (shift k k' s).
-Proof. intros; now apply shift_preserves_valid_1. Qed.
+Theorem shift_preserves_wf (m n: Lvl.t) (s: t) :
+  Wf m s -> Wf (m + n) (shift m n s).
+Proof. intros; now apply shift_preserves_wf_1. Qed.
 
-Lemma shift_preserves_valid_zero : forall k t, valid k t -> valid k (shift k 0 t).
-Proof. intros; replace k with (k + 0); try lia; now apply shift_preserves_valid_1. Qed.
+Lemma shift_preserves_wf_zero (m: Lvl.t) (s: t) : Wf m s -> Wf m (shift m 0 s).
+Proof. intros; replace m with (m + 0); try lia; now apply shift_preserves_wf_1. Qed.
 
-Lemma shift_preserves_valid_gen : forall lb lb' k k' t,
-  k <= k' -> lb <= lb' -> k <= lb -> k' <= lb' -> k' - k = lb' - lb -> 
-  valid lb t -> valid lb' (shift k (k' - k) t).
+Lemma shift_preserves_wf_gen (m m' n k: Lvl.t) (s: t) :
+  n <= k -> m <= m' -> n <= m -> k <= m' -> k - n = m' - m -> 
+  Wf m s -> Wf m' (shift n (k - n) s).
 Proof.
-  unfold valid,For_all in *; intros. apply shift_in_e_spec in H5. 
+  unfold Wf,For_all in *; intros. apply shift_in_e in H5. 
   destruct H5 as [y [Heq HIn]]; subst.
-  apply T.shift_preserves_valid_gen with (lb := lb); auto.
+  apply T.shift_preserves_wf_gen with (m := m); auto.
   apply H4. now rewrite <- shift_in_iff in HIn.
 Qed.
 
-Lemma shift_preserves_valid_2 : forall lb lb' t,
-  lb <= lb' -> valid lb t -> 
-  valid lb' (shift lb (lb' - lb) t).
-Proof. intros. eapply shift_preserves_valid_gen; eauto. Qed.
+Lemma shift_preserves_wf_2 (m n: Lvl.t) (s: t) :
+  m <= n -> Wf m s -> 
+  Wf n (shift m (n - m) s).
+Proof. intros. eapply shift_preserves_wf_gen; eauto. Qed.
 
 End IsLvlSet.
 
-(** ** Bindless Leveled Map Implementation *)
+
+(** ---- *)
+
+
+(** ** Leveled Set Implementation - [OT], [BD] and [WL] *)
 Module IsBdlLvlSet (T : IsBdlLvlOTWL) (Import Se : SetOTWithLeibnizInterface T) <: IsBdlLvlOTWL.
 
 Include IsLvlSet T Se.
 
-Lemma shift_valid_refl : forall lb k s,
-  valid lb s -> eq (shift lb k s) s.
+Lemma shift_wf_refl (m n: Lvl.t) (s: t) :
+  Wf m s -> eq (shift m n s) s.
 Proof.
-  intros lb k s; induction s using set_induction; intros.
+  induction s using set_induction; intros.
   - apply empty_is_empty_1 in H; apply eq_leibniz in H; subst.
-    now rewrite shift_empty_spec.
+    now rewrite shift_empty.
   
   - apply Add_inv in H0; subst.
-    rewrite shift_add_notin_spec; try assumption.
-    apply valid_add_spec in H1; destruct H1; f_equal.
-    rewrite T.shift_valid_refl; auto.
+    rewrite shift_add_notin; try assumption.
+    apply Wf_add_iff in H1; destruct H1; f_equal.
+    rewrite T.shift_wf_refl; auto.
     apply IHs1 in H1; now rewrite H1.
+Qed.
+
+Lemma Wf_in_iff (m n : Lvl.t) (r : elt) (s : t):
+  Wf m s -> In r (shift m n s) <-> In r s.
+Proof.
+  induction s using set_induction; intro Hv; split.
+  - intro HIn; rewrite shift_Empty in *; auto; inversion HIn.
+  - intro HIn; unfold Empty in *; exfalso; now apply (H r).
+  - intro HIn; apply Add_inv in H0; subst. rewrite shift_add_notin in *; auto.
+    apply Wf_add_iff in Hv as [Hvr Hv]. rewrite add_spec in HIn; destruct HIn; subst.
+    -- rewrite H0. rewrite T.shift_wf_refl; auto; rewrite add_spec; now left.
+    -- rewrite add_spec; right. rewrite <- IHs1; eauto.
+  - intro HIn; apply Add_inv in H0; subst. rewrite shift_add_notin in *; auto.
+    apply Wf_add_iff in Hv as [Hvr Hv]. rewrite add_spec in HIn; destruct HIn; subst.
+    -- rewrite H0. rewrite T.shift_wf_refl; auto; rewrite add_spec; now left.
+    -- rewrite add_spec; right. rewrite IHs1; eauto.
 Qed.
 
 End IsBdlLvlSet.
 
-(** ** Leveled Map Implementation with [validb] *)
+
+(** ---- *)
+
+
+(** ** Leveled Set Implementation - [OT], [FL] and [WL] *)
 Module IsLvlFullSet 
   (T : IsLvlFullOTWL) (Import Se : SetOTWithLeibnizInterface T) <: IsLvlFullSetInterface T Se.
 
 Include IsLvlSet T Se.
 
-Definition validb (k : nat) (s : t) := (for_all (fun v => T.validb k v) s).
+Definition is_wf (n : Lvl.t) (s : t) := (for_all (fun v => T.is_wf n v) s).
 
-#[export]
-Instance proper_valid : Proper (Logic.eq ==> T.eq ==> Logic.eq) T.validb.
-Proof. repeat red; intros; subst. apply T.eq_leibniz in H0; now subst. Qed.
-
-Lemma validb_valid : forall k t, validb k t = true <-> valid k t. 
+Lemma Wf_is_wf_true (m: Lvl.t) (s: t) : Wf m s <-> is_wf m s = true. 
 Proof.
-  unfold valid,validb; split; intros; rewrite for_all_spec in *; unfold For_all in *;
+  unfold Wf,is_wf; split; intros; rewrite for_all_spec in *; unfold For_all in *;
   try (repeat red; intros; now subst); auto.
-  - intros; rewrite <- T.validb_valid; auto.
+  - intros; rewrite <- T.Wf_is_wf_true; auto.
   - repeat red; intros; subst. apply T.eq_leibniz in H0; now subst.
-  - intros; rewrite T.validb_valid; auto.
+  - intros; rewrite T.Wf_is_wf_true; auto.
   - repeat red; intros; subst. apply T.eq_leibniz in H0; now subst.
 Qed.
 
-Lemma validb_nvalid : forall k t, validb k t = false <-> ~ valid k t.
+Lemma notWf_is_wf_false (m: Lvl.t) (s: t) : ~ Wf m s <-> is_wf m s = false.
 Proof.
   intros; rewrite <- not_true_iff_false; split; intros; intro.
-  - apply H; now rewrite validb_valid. 
-  - apply H; now rewrite <- validb_valid.
+  - apply H; now rewrite Wf_is_wf_true. 
+  - apply H; now rewrite <- Wf_is_wf_true.
 Qed.
 
-#[export]
-Instance validb_eq : Proper (Logic.eq ==> eq ==> Logic.eq) validb.
+#[export] Instance is_wf_eq : Proper (Logic.eq ==> eq ==> Logic.eq) is_wf.
 Proof. repeat red; intros; subst; apply eq_leibniz in H0; now subst. Qed.
 
 End IsLvlFullSet.
 
-(** ** Bindless Leveled Map Implementation with [validb] *)
+
+(** ---- *)
+
+
+(** ** Leveled Set Implementation - [OT], [FL], [BD] and [WL] *)
 Module IsBdlLvlFullSet (T : IsBdlLvlFullOTWL) 
-  (Import Se : SetOTWithLeibnizInterface T) <: IsBdlLvlFullSetInterface T Se.
+                       (Import Se : SetOTWithLeibnizInterface T) <: IsBdlLvlFullSetInterface T Se.
 
 Include IsLvlFullSet T Se.
 
-Lemma shift_valid_refl : forall lb k s,
-  valid lb s -> eq (shift lb k s) s.
+Lemma shift_wf_refl (m n: Lvl.t) (s: t) :
+  Wf m s -> eq (shift m n s) s.
 Proof.
-  intros lb k s; induction s using set_induction; intros.
+  induction s using set_induction; intros.
   - apply empty_is_empty_1 in H; apply eq_leibniz in H; subst.
-    now rewrite shift_empty_spec.
+    now rewrite shift_empty.
   
   - apply Add_inv in H0; subst.
-    rewrite shift_add_notin_spec; try assumption.
-    apply valid_add_spec in H1; destruct H1; f_equal.
-    rewrite T.shift_valid_refl; auto.
+    rewrite shift_add_notin; try assumption.
+    apply Wf_add_iff in H1; destruct H1; f_equal.
+    rewrite T.shift_wf_refl; auto.
     apply IHs1 in H1; now rewrite H1.
+Qed.
+
+Lemma Wf_in_iff (m k: Lvl.t) (r: elt) (s: t) :
+  Wf m s -> In r (shift m k s) <-> In r s.
+Proof.
+  induction s using set_induction; intro Hv; split.
+  - intro HIn; rewrite shift_Empty in *; auto; inversion HIn.
+  - intro HIn; unfold Empty in *; exfalso; now apply (H r).
+  - intro HIn; apply Add_inv in H0; subst. rewrite shift_add_notin in *; auto.
+    apply Wf_add_iff in Hv as [Hvr Hv]. rewrite add_spec in HIn; destruct HIn; subst.
+    -- rewrite H0. rewrite T.shift_wf_refl; auto; rewrite add_spec; now left.
+    -- rewrite add_spec; right. rewrite <- IHs1; eauto.
+  - intro HIn; apply Add_inv in H0; subst. rewrite shift_add_notin in *; auto.
+    apply Wf_add_iff in Hv as [Hvr Hv]. rewrite add_spec in HIn; destruct HIn; subst.
+    -- rewrite H0. rewrite T.shift_wf_refl; auto; rewrite add_spec; now left.
+    -- rewrite add_spec; right. rewrite IHs1; eauto.
 Qed.
 
 End IsBdlLvlFullSet.
 
+
 (** ---- *)
+
 
 (** * Make - Leveled Set *)
 
