_TMP/Map/Maps/MapLvlD.v
@@ -1,0 +1,284 @@
+From Coq Require Import Lia Arith.PeanoNat Classical_Prop Classes.RelationClasses.
+From MMaps Require Import MMaps.
+From DeBrLevel Require Import Level LevelInterface MapExtInterface MapExt MapLevelInterface MapKD.
+
+(** * Implementation - Map - [LevelK/LvlD] *)
+
+(** ** Leveled Map Implementation *)
+
+Module IsLvlMapLVLD
+  (Data : IsLvlETWL) (M : Interface.S Level) 
+  (MO : MapLVLInterface Data M) <: IsLvlMapLVLDInterface Data M MO.
+
+Include IsLvlMapKD Level Data M MO.
+Import MO OP.P.
+
+Lemma shift_new_notin_spec (lb k : Lvl.t) (t : t) :
+  lb >= (new_key t) -> ~ M.In lb (shift lb k t).
+Proof.
+  induction t using map_induction; intros Hgeq.
+  - rewrite shift_Empty_spec; auto.
+    rewrite Empty_eq_spec; auto.
+    apply not_in_empty.
+  - unfold Add in *; rewrite H0 in *; clear H0.
+    rewrite shift_add_notin_spec; auto. 
+    rewrite add_in_iff.
+    intros [Heq | HIn].
+    -- unfold Level.shift in Heq. 
+       destruct (Nat.leb_spec0 lb x) as [Hle | Hnle].
+       + assert (HIn : M.In x (M.add x e t1)).
+         { exists e. now apply add_1. }
+         assert (HnIn : ~ M.In x (M.add x e t1)). 
+         { apply new_key_notin_spec; lia. }
+         contradiction.
+        + subst; lia.
+    -- revert HIn; apply IHt1. 
+       apply new_key_add_spec with (v := e) in H; auto.
+       destruct H as [[Heq Hleb] | [Heq Hgt]]; try lia.
+Qed.
+
+Lemma shift_max_refl_spec (lb k : Lvl.t) (t : t) :
+  lb >= (new_key t) -> max_key (shift lb k t) = max_key t.
+Proof.
+  induction t using map_induction; intros Hle.
+  - rewrite shift_Empty_spec; auto.
+  - unfold Add in *; rewrite H0 in *; clear H0.
+    rewrite shift_add_spec.
+    apply max_key_add_spec with (v := e) in H as HI. 
+    assert (Hge : lb >= new_key t1).
+    {
+        apply new_key_add_spec with (v := e) in H; auto.
+        destruct H as [[Heq Hleb'] | [Heq Hgt]]; lia.
+    }
+
+    destruct HI as [[Heq Hleb] | [Heq Hgt]].
+    -- rewrite new_key_add_ge_spec in Hle; auto.
+       + rewrite Heq.
+         rewrite max_key_add_ge_spec; auto.
+         * apply Level.shift_valid_refl.
+           unfold Level.valid; lia.
+         * now rewrite <- shift_notin_iff.
+         * rewrite IHt1; try lia.
+           rewrite Level.shift_valid_refl; auto.
+       + rewrite new_key_unfold.
+         destruct (M.is_empty t1); lia.
+    -- assert (Hlt : x < lb).
+       {
+         transitivity (max_key t1); try lia.
+         rewrite <- Heq.
+         rewrite new_key_unfold in Hle.
+         destruct (M.is_empty (M.add x e t1)) eqn:Hemp; try lia.
+         apply is_empty_2 in Hemp.
+         exfalso.
+         apply (Hemp x e).
+         now apply add_1.
+       } 
+       rewrite new_key_add_lt_spec in Hle; auto.
+       + rewrite Heq.
+         rewrite max_key_add_lt_spec; auto.
+         * now rewrite <- shift_notin_iff.
+         * rewrite IHt1; auto.
+           rewrite Level.shift_valid_refl; auto.
+       + rewrite new_key_unfold.
+         destruct (M.is_empty t1) eqn:Hemp; try lia.
+         rewrite max_key_Empty_spec in Hgt; try lia.
+         now apply is_empty_2.
+Qed.
+
+Lemma shift_new_refl_spec (lb k : Lvl.t) (t : t) :
+  lb >= (new_key t) -> new_key (shift lb k t) = new_key t.
+Proof.
+  repeat rewrite new_key_unfold; intro Hge.
+  destruct (M.is_empty t) eqn:Hemp.
+  - apply is_empty_2 in Hemp as HEmp.
+    rewrite (shift_Empty_iff lb k) in HEmp.
+    apply is_empty_1 in HEmp.
+    now rewrite HEmp.
+  - destruct (M.is_empty (shift lb k t)) eqn:Hemp'.
+    -- apply is_empty_2 in Hemp'. 
+       rewrite <- shift_Empty_iff in Hemp'.
+       apply is_empty_1 in Hemp'. 
+       rewrite Hemp in *; inversion Hemp'.
+    -- f_equal; apply shift_max_refl_spec.
+       rewrite new_key_unfold.
+       now rewrite Hemp.
+Qed.  
+
+Lemma shift_max_key_gt_iff (m n x : Lvl.t) (o : t) :
+  max_key o > x <-> max_key (shift m n o) > (Level.shift m n x).
+Proof.
+  revert x; induction o using map_induction; intro y.
+  - split; intro Hmax.
+    -- rewrite max_key_Empty_spec in Hmax; auto; lia.
+    -- rewrite shift_Empty_spec in Hmax; auto.
+       rewrite max_key_Empty_spec in Hmax; auto; lia.
+  - split; intro Hmax;
+    unfold Add in H0; rewrite H0 in *; clear H0.
+    -- destruct (Level.leb_spec (max_key o1) x) as [Hle | Hgt].
+       + rewrite max_key_add_ge_spec in Hmax; auto; try lia.
+         rewrite shift_add_spec.
+         rewrite (shift_in_iff m n) in H.
+         destruct (Level.leb_spec (max_key (shift m n o1)) (Level.shift m n x)) as [Hle' | Hgt'].
+         ++ rewrite max_key_add_ge_spec; auto; try lia.
+            now apply Level.shift_gt_iff.
+         ++ rewrite max_key_add_lt_spec; auto; try lia.
+            assert (max_key o1 > x) by (rewrite IHo1; lia); lia.
+       + rewrite max_key_add_lt_spec in Hmax; auto; try lia.
+         rewrite shift_add_spec.
+         rewrite (shift_in_iff m n) in H.
+         destruct (Level.leb_spec (max_key (shift m n o1)) (Level.shift m n x)) as [Hle' | Hgt'].
+         ++ rewrite IHo1 in Hmax.
+            rewrite max_key_add_ge_spec; auto; lia.
+         ++ rewrite max_key_add_lt_spec; auto; try lia.
+            now rewrite <- IHo1.
+    -- rewrite shift_add_spec in Hmax.
+       rewrite (shift_in_iff m n) in H.
+       destruct (Level.leb_spec (max_key (shift m n o1)) (Level.shift m n x)) as [Hle | Hgt].
+       + rewrite max_key_add_ge_spec in Hmax; auto; try lia.
+         rewrite <- (shift_in_iff m n) in H.
+         destruct (Level.leb_spec (max_key o1) x) as [Hle' | Hgt'].
+         ++ rewrite max_key_add_ge_spec; auto; try lia.
+            now apply Level.shift_gt_iff in Hmax.
+         ++ rewrite max_key_add_lt_spec; auto; try lia.
+            rewrite <- Level.shift_gt_iff in Hmax; lia.
+       + rewrite max_key_add_lt_spec in Hmax; auto; try lia.
+         rewrite <- (shift_in_iff m n) in H.
+         destruct (Level.leb_spec (max_key o1) x) as [Hle' | Hgt'].
+         ++ rewrite max_key_add_ge_spec; auto; try lia.
+            rewrite <- IHo1 in Hmax; lia.
+         ++ rewrite max_key_add_lt_spec; auto; try lia.
+            rewrite <- IHo1 in Hmax; lia.
+Qed. 
+
+Lemma shift_max_key_le_spec (m n : Lvl.t) (o : t) :
+  max_key o <= max_key (shift m n o).
+Proof.
+  induction o using map_induction.
+  - now rewrite shift_Empty_spec.
+  - unfold Add in H0; rewrite H0; clear H0. 
+    rewrite shift_add_spec.
+    destruct (Level.leb_spec (max_key o1) x) as [Hle | Hgt].
+    -- rewrite max_key_add_ge_spec; auto; try lia.
+       rewrite (shift_in_iff m n) in H.
+       destruct (Level.leb_spec (max_key (shift m n o1)) (Level.shift m n x)) as [Hle' | Hgt'].
+       + rewrite max_key_add_ge_spec; auto; try lia.
+         apply Level.shift_le_spec.
+       + rewrite max_key_add_lt_spec; auto; try lia.
+         assert (Hgt : max_key (shift m n o1) > Level.shift m n x) by lia.
+         rewrite <- shift_max_key_gt_iff in Hgt; lia.
+    -- rewrite max_key_add_lt_spec; auto; try lia.
+       rewrite (shift_in_iff m n) in H.
+       destruct (Level.leb_spec (max_key (shift m n o1)) (Level.shift m n x)) as [Hle' | Hgt'].
+       + rewrite max_key_add_ge_spec; auto; lia.
+       + rewrite max_key_add_lt_spec; auto; lia.
+Qed.
+       
+Lemma shift_new_key_le_spec (m n : Lvl.t) (o : t) :
+  new_key o <= new_key (shift m n o).
+Proof.
+  repeat rewrite new_key_unfold.
+  destruct (M.is_empty o) eqn:Hemp; try lia.
+  destruct (M.is_empty (shift m n o)) eqn:Hemp'.
+  - apply is_empty_2 in Hemp'. 
+    rewrite <- (shift_Empty_iff m n) in Hemp'.
+    apply is_empty_1 in Hemp'.
+    rewrite Hemp in Hemp'; now inversion Hemp'.
+  - assert (max_key o <= max_key (shift m n o)); try lia.
+    apply shift_max_key_le_spec.
+Qed.
+
+Lemma valid_in_iff (m n : Lvl.t) (x : M.key) (t : t) :
+  valid m t -> M.In x (shift m n t) <-> M.In x t.
+Proof.
+  revert x; induction t using map_induction; intros y Hvo; split; intro HIn.
+  - rewrite shift_Empty_spec in HIn; auto.
+  - rewrite shift_Empty_spec; auto.
+  - unfold Add in *; rewrite H0 in *; clear H0. 
+    apply valid_add_notin_spec in Hvo as [Hvk [Hve Hv]]; auto.
+    rewrite shift_add_notin_spec in HIn; auto.
+    rewrite add_in_iff in *; destruct HIn as [Heq | HIn]; subst.
+    -- left; now rewrite Level.shift_valid_refl; auto.
+    -- right. rewrite <- IHt1; eauto.
+  - unfold Add in *; rewrite H0 in *; clear H0. 
+    apply valid_add_notin_spec in Hvo as [Hvk [Hve Hv]]; auto.
+    rewrite shift_add_notin_spec; auto.
+    rewrite add_in_iff in *; destruct HIn as [Heq | HIn]; subst.
+    -- left; now rewrite Level.shift_valid_refl; auto.
+    -- right. rewrite IHt1; eauto.
+Qed.
+
+Lemma shift_find_valid_spec (lb k : Lvl.t) (x : M.key) (m m' : t) :
+  Level.valid lb x -> M.In x m ->
+  M.find x m = M.find x m' -> M.find x (shift lb k m) = M.find x (shift lb k m').
+Proof.
+  intros Hvk HIn Hfi. 
+  destruct HIn as [v HfV]; apply find_1 in HfV.
+  rewrite <- (Level.shift_valid_refl lb k x); auto.
+  apply (shift_find_iff lb k) in HfV as HfV1.
+  rewrite HfV1; symmetry.
+  rewrite <- shift_find_iff.
+  now rewrite <- Hfi.
+Qed.
+
+Lemma shift_in_new_key (n : Lvl.t) (x : M.key) (t : t) :
+  M.In x (shift (new_key t) n t) <-> M.In x t.
+Proof.
+  split; intro HIn.
+  - apply shift_in_e_spec in HIn as H.
+    destruct H as [y Heq]; subst.
+    rewrite <- shift_in_iff in HIn.
+    apply new_key_in_spec in HIn as Hlt.
+    rewrite Level.shift_valid_refl; auto.
+  - apply new_key_in_spec in HIn as Hlt.
+    rewrite <- (Level.shift_valid_refl (new_key t) n x); auto.
+    now rewrite <- shift_in_iff.
+Qed.
+
+End IsLvlMapLVLD.
+
+(** ** Bindless Leveled Map Implementation *)
+Module IsBdlLvlMapLVLD 
+  (Data : IsBdlLvlETWL) (M : Interface.S Level) 
+  (MO : MapLVLInterface Data M) <: IsBdlLvlMapLVLDInterface Data M MO.
+
+Include IsLvlMapLVLD Data M MO.
+Import MO OP.P.
+
+Lemma shift_valid_refl (lb k : Lvl.t) (t : t) : valid lb t -> eq (shift lb k t) t.
+Proof.
+  induction t using map_induction; intro Hvt.
+  - now apply shift_Empty_spec.
+  - unfold Add in H0; rewrite H0 in *; clear H0.
+    apply valid_add_notin_spec in Hvt as [Hvx [Hve Hvt]]; auto. 
+    rewrite shift_add_spec.
+    rewrite IHt1; auto.
+    rewrite Level.shift_valid_refl; auto.
+
+    replace (Data.shift lb k e) with e; try reflexivity.
+    apply Data.eq_leibniz.
+    now rewrite Data.shift_valid_refl; auto.
+Qed.
+    
+End IsBdlLvlMapLVLD.
+
+
+(** *** Map Make *)
+
+Module MakeLvlMapLVLD (Data : IsLvlETWL) <: IsLvlET.
+  
+  Module Raw := MMaps.OrdList.Make Level.
+  Module Ext := MapETLVL Data Raw.
+  Include IsLvlMapLVLD Data Raw Ext.
+  Include OP.P.
+
+End MakeLvlMapLVLD.
+
+
+Module MakeBdlLvlMapLVLD (Data : IsBdlLvlETWL) <: IsBdlLvlET.
+  
+  Module Raw := MMaps.OrdList.Make Level.
+  Module Ext := MapETLVL Data Raw.
+  Include IsBdlLvlMapLVLD Data Raw Ext.
+  Include OP.P.
+
+End MakeBdlLvlMapLVLD.
