theories/Core/LevelInterface.v
@@ -3,157 +3,113 @@ Import Structures.Equalities Structures.Orders.
 
 (** * Interface - Level 
 
-  De-Bruijn has proposed a variation of the lambda calculus which instanciates variables
-  in a determinisc way. It defines two measures: the distance and the level. The distance,
-  latter called index, is the number of abstraction between a variable and its binder. The
-  level is the number of abstraction encountered since the root of the representative tree
-  of a term.
+  De-Bruijn has proposed a variation of the lambda calculus which instanciates variables in a determinisc way. It defines two measures: the distance and the level. The distance, latter called index, is the number of abstraction between a variable and its binder. The level is the number of abstraction encountered since the root of the representative tree of a term.
 
-  For instance, λx.(λy.(x y) x) is equal to λ.(λ.(1 0) 0) with distances and λ.(λ.(0 1) 0) 
-  with levels.
+  For instance, λx.(λy.(x y) x) is equal to λ.(λ.(1 0) 0) with distances and λ.(λ.(0 1) 0) with levels.
 
-  This kind of representations are extremely simple and can be used in different context as
-  well as be embedded in data types or data structures.
+  This kind of representations are extremely simple and can be used in different context as well as be embedded in data types or data structures.
 *)
 
 (** ** Level - Definition
 
-  A level itself only require to be ordered. We require also a ground value and
-  classic arithmetic operators on it. Thus, we define a level as a [Nat].
+  A level itself only requires to be ordered. We require also a ground value and classic arithmetic operators on it. Thus, we define a level as a [Nat].
 
 *)
 Module Lvl <: Orders.OrderedTypeFull := Structures.OrdersEx.Nat_as_OT.
 
 (** ---- *)
 
-(** ** Valid and Shift interfaces 
+(** ** Well-formedness and Shift interfaces 
 
-  We split the definition of an element that used levels in different module types.
-  First, we want to be as flexible as possible. Second, each modules types carries
-  an additional set of constraints.
+  We split the definition of an element that used levels in different module types. First, we want to be as flexible as possible. Second, each modules types carries an additional set of constraints.
 
-  We define a function called [shift] and a property called [valid]. It is the minimal set
-  of elements for working with levels. Their principles ared defined below.
+  We define a function called [shift] and a property called [Wf]. It is the minimal set of elements for working with levels. Their principles ared defined below.
 *)
 
-(** *** Valid Property
+(** *** Well-formedness
 
-  If we define an inductive type as containing levels, the questioning about the well-formation or ill-formation appears.
-  Thus we suppose a property [valid], to define by the user, which is satisfied if the instanciation is well formed.
+  If we define an inductive type as containing levels, the questioning about the well-formation or ill-formation appears. Thus we suppose a property [Wf], defined by the user later, which is satisfied if the instanciation is well-formed.
 
-  What is a well formed type ? If we take the most basic case, a level, when can we state that a level is valid or not ?
-  We can only talk about a valid level regards of a lower bound [lb]. 
+  What is a well-formed type? If we take the most basic case, a level, when can we state that a level is well-formed or not ? We can only talk about a well-formed level regards of a lower bound [m]. 
 
-  We use the case of the lambda calculus to illustrate it. Consider the term "x", the variable is free. Thus, how do we state
-  that it is a well formed term ? We suppose that "x" is defined in a certain context. Now, consider the term "λx.(x y)". "y" is 
-  free and "x" bound. The term is well formed if "y" is defined in a certain context. The lower bound can be here understood as 
+  We use the case of the lambda calculus to illustrate it. Consider the term "x", the variable is free. Thus, how do we state that it is a well-formed term? We suppose that "x" is defined in a certain context. Now, consider the term "λx.(x y)". "y" is free and "x" bound. The term is well-formed if "y" is defined in a certain context. The lower bound can be here understood as 
   the number of free variables.
-
 *)
 
-(** **** [valid] property interface *)
-Module Type HasValid (Import T : EqualityType).
+(** **** [Wf] property interface *)
+Module Type IsWF (Import T : EqualityType).
 
-Section operation.
+Parameter Wf : Lvl.t -> t -> Prop.
 
-Parameter valid : Lvl.t -> t -> Prop.
+Parameter Wf_weakening : forall (m n: Lvl.t) (t: t), Lvl.le m n -> Wf m t -> Wf n t.
 
-End operation.
+#[export] Declare Instance Wf_iff : Proper (Lvl.eq ==> eq ==> iff) Wf.
 
-Section properties.
-
-Variable k k' : Lvl.t.
-Variable t : t.
-  
-Parameter valid_weakening : Lvl.le k k' -> valid k t -> valid k' t.
-
-#[export] Declare Instance valid_eq : Proper (Lvl.eq ==> eq ==> iff) valid.
-
-End properties.
-
-End HasValid.
+End IsWF.
 
 
-(** **** Boolean version of [valid] named [validb] *)
-Module Type HasValidb (Import T : EqualityType).
+(** **** Boolean version of [Wf] named [is_wf] *)
+Module Type IsWFb (Import T : EqualityType).
 
-Section operation.
+Parameter is_wf : Lvl.t -> t -> bool.
 
-Parameter validb : Lvl.t -> t -> bool.
+#[export] Declare Instance is_wf_eq : Proper (Lvl.eq ==> eq ==> Logic.eq) is_wf.
 
-End operation.
+End IsWFb.
 
-Section properties.
+(** **** [Wf] property with its boolean version [is_wf] *)
+Module Type IsWFFull (Import T : EqualityType) (Import V : IsWF T) <: IsWFb T.
 
-#[export] Declare Instance validb_eq : Proper (Lvl.eq ==> eq ==> Logic.eq) validb.
+Include IsWFb T.
 
-End properties.
-
-End HasValidb.
-
-(** **** [valid] property with its boolean version [validb] *)
-Module Type HasValidFull (Import T : EqualityType) (Import V : HasValid T) <: HasValidb T.
-
-Include HasValidb T.
-
-Section properties.
+Section specifications.
 
 Variable k : Lvl.t.
 Variable t : t.
 
-Parameter validb_valid  : validb k t = true  <->   valid k t. 
-Parameter validb_nvalid : validb k t = false <-> ~ valid k t. 
+Parameter Wf_is_wf_true : Wf k t <-> is_wf k t = true. 
+Parameter notWf_is_wf_false : ~ Wf k t <-> is_wf k t = false. 
 
-End properties.
+End specifications.
 
-End HasValidFull.
+End IsWFFull.
 
 (** ***  Shift function
 
-  Like indices, we will often shift levels. Consequently, we ask to the user to define a [shift] function. This function 
-  takes three arguments: the lower bound [lb], the shift [k] and the leveled element [t]. The lower bound has the same 
-  meaning that the one in the [valid] property. In lambda calculus, we can say that we shift only bound variables knowing
-  a certain number of free variables. It is a main difference with indices. Indeed, free variables have a fix level 
-  defined. Thus, no need to shift them.
-  For instance, the shift function interacts as shown below with the levels.
+  Like indices, we will often shift levels. Consequently, we ask to the user to define a [shift] function. This function takes three arguments: the lower bound [m], the shift [k] and the leveled element [t]. The lower bound has the same meaning that the one in the [Wf] property. In lambda calculus, we can say that we shift only bound variables knowing a certain number of free variables. It is a main difference with indices. Indeed, free variables have a fix level defined. Thus, no need to shift them. For instance, the shift function interacts as shown below with the levels.
 <<
 shift 0 2 2 = 4
 shift 3 2 2 = 2
 shift 65 0 98 = 98
 >>
 
-  In a lambda calculus term, we can see the use of [lb].
+  In a lambda calculus term, we can see the use of [m].
 <<
 shift 1 3 (\. 0 1) = (\. 0 4)
 >>
 *)
 
-(** **** [shift] function property *)
+(** **** [shift] function interface *)
 Module Type HasShift (Import T : EqualityType).
-
-Section operation.
 
 Parameter shift : Lvl.t -> Lvl.t -> t -> t.
 
-End operation.
+Section specifications.
 
-Section properties.
-
-Variable lb k k' k'' : Lvl.t.
+Variable m n k p : Lvl.t.
 Variable t t' : t.
 
-Parameter shift_zero_refl : eq (shift lb 0 t) t.
-Parameter shift_trans     : eq (shift lb k (shift lb k' t)) (shift lb (k + k') t).
-Parameter shift_permute   : eq (shift lb k (shift lb k' t)) (shift lb k' (shift lb k t)).
-Parameter shift_unfold    : eq (shift lb (k + k') t) (shift (lb + k) k' (shift lb k t)). 
-Parameter shift_unfold_1  :
-  k <= k' -> k' <= k'' -> eq (shift k' (k'' - k') (shift k  (k' - k) t)) (shift k (k'' - k) t).
+Parameter shift_zero_refl : eq (shift m 0 t) t.
+Parameter shift_trans     : eq (shift m n (shift m k t)) (shift m (n + k) t).
+Parameter shift_permute   : eq (shift m n (shift m k t)) (shift m k (shift m n t)).
+Parameter shift_unfold    : eq (shift m (n + k) t) (shift (m + n) k (shift m n t)). 
+Parameter shift_unfold_1  : n <= k -> k <= p -> 
+                            eq (shift k (p - k) (shift n  (k - n) t)) (shift n (p - n) t).
+Parameter shift_eq_iff    : eq t t' <-> eq (shift m k t) (shift m k t').
 
-#[export] 
-Declare Instance shift_eq : Proper (Lvl.eq ==> Lvl.eq ==> eq ==> eq) shift.
-Parameter shift_eq_iff    : eq t t' <-> eq (shift lb k t) (shift lb k t').
+#[export] Declare Instance shift_eq : Proper (Lvl.eq ==> Lvl.eq ==> eq ==> eq) shift.
 
-End properties.
+End specifications.
 
 End HasShift.
 
@@ -165,24 +121,24 @@ End HasShift.
   A type [t] that uses levels have to implements this module type.
 
 *)
-Module Type IsLeveled (Import T : EqualityType) <: HasShift T <: HasValid T.
+Module Type IsLeveled (Import T : EqualityType) <: HasShift T <: IsWF T.
 
-Include HasShift T <+ HasValid T.
+Include HasShift T <+ IsWF T.
 
-Section properties.
+Section specifications.
 
-  Variable lb lb' k k' : Lvl.t.
-  Variable t : t.
+Variable m n k p : Lvl.t.
+Variable t : t.
 
-  Parameter shift_preserves_valid_gen :  
-    k <= k' -> lb <= lb' -> k <= lb -> k' <= lb' -> k' - k = lb' - lb ->
-    valid lb t -> valid lb' (shift k (k' - k) t).
-  Parameter shift_preserves_valid   : valid k t -> valid (k + k') (shift k k' t).
-  Parameter shift_preserves_valid_1 : valid k t -> valid (k + k') (shift lb k' t).
-  Parameter shift_preserves_valid_2 : lb <= lb' -> valid lb t -> valid lb' (shift lb (lb' - lb) t).
-  Parameter shift_preserves_valid_zero : valid k t -> valid k (shift k 0 t).
+Parameter shift_preserves_wf_gen :
+  k <= p -> m <= n -> k <= m -> p <= n -> p - k = n - m ->
+  Wf m t -> Wf n (shift k (p - k) t).
+Parameter shift_preserves_wf   : Wf k t -> Wf (k + p) (shift k p t).
+Parameter shift_preserves_wf_1 : Wf k t -> Wf (k + p) (shift m p t).
+Parameter shift_preserves_wf_2 : m <= n -> Wf m t -> Wf n (shift m (n - m) t).
+Parameter shift_preserves_wf_zero : Wf k t -> Wf k (shift k 0 t).
 
-End properties.
+End specifications.
 
 End IsLeveled.
 
@@ -190,7 +146,7 @@ End IsLeveled.
 (** ** Bindless Leveled Module Type
 
   A type [t] that uses levels without binders has a specific property. The [shift] function did not
-  impact the type if it shares the same lower bound with the [valid] property.
+  impact the type if it shares the same lower bound with the [Wf] property.
   This kind of types is common actually. A set, a map or a pair does not imply binders.
 
 *)
@@ -198,13 +154,13 @@ Module Type IsBindlessLeveled (Import T : EqualityType) <: IsLeveled T.
 
 Include IsLeveled T.
 
-Parameter shift_valid_refl : forall lb k t, valid lb t -> eq (shift lb k t) t.
+Parameter shift_wf_refl : forall m k t, Wf m t -> eq (shift m k t) t.
 
 End IsBindlessLeveled.
 
 Module Type IsBindlessLeveledEx (Import T : EqualityType) (Import IsLvl : IsLeveled T).
 
-Parameter shift_valid_refl : forall lb k t, valid lb t -> eq (shift lb k t) t.
+Parameter shift_wf_refl : forall m k t, Wf m t -> eq (shift m k t) t.
 
 End IsBindlessLeveledEx.
 
@@ -262,10 +218,10 @@ Module Type IsLeveledETWithLeibniz := EqualityTypeWithLeibniz <+ IsLeveled.
 Module Type IsBindlessLeveledET :=  EqualityType <+ IsBindlessLeveled.
 Module Type IsBindlessLeveledETWithLeibniz := EqualityTypeWithLeibniz <+ IsBindlessLeveled.
 
-Module Type IsLeveledFullET := IsLeveledET <+ HasValidFull.
-Module Type IsLeveledFullETWithLeibniz := IsLeveledETWithLeibniz <+ HasValidFull.
-Module Type IsBindlessLeveledFullET := IsBindlessLeveledET <+ HasValidFull.
-Module Type IsBindlessLeveledFullETWithLeibniz := IsBindlessLeveledETWithLeibniz <+ HasValidFull.
+Module Type IsLeveledFullET := IsLeveledET <+ IsWFFull.
+Module Type IsLeveledFullETWithLeibniz := IsLeveledETWithLeibniz <+ IsWFFull.
+Module Type IsBindlessLeveledFullET := IsBindlessLeveledET <+ IsWFFull.
+Module Type IsBindlessLeveledFullETWithLeibniz := IsBindlessLeveledETWithLeibniz <+ IsWFFull.
 
 Module Type IsLvlET := IsLeveledET.
 Module Type IsLvlETWL := IsLeveledETWithLeibniz.
@@ -286,10 +242,10 @@ Module Type IsLeveledDTWithLeibniz := DecidableTypeWithLeibniz <+ IsLeveled.
 Module Type IsBindlessLeveledDT :=  EqualityType <+ HasEqDec <+ IsBindlessLeveled.
 Module Type IsBindlessLeveledDTWithLeibniz := DecidableTypeWithLeibniz <+ IsBindlessLeveled.
 
-Module Type IsLeveledFullDT := IsLeveledDT <+ HasValidFull.
-Module Type IsLeveledFullDTWithLeibniz := IsLeveledDTWithLeibniz <+ HasValidFull.
-Module Type IsBindlessLeveledFullDT := IsBindlessLeveledDT <+ HasValidFull.
-Module Type IsBindlessLeveledFullDTWithLeibniz := IsBindlessLeveledDTWithLeibniz <+ HasValidFull.
+Module Type IsLeveledFullDT := IsLeveledDT <+ IsWFFull.
+Module Type IsLeveledFullDTWithLeibniz := IsLeveledDTWithLeibniz <+ IsWFFull.
+Module Type IsBindlessLeveledFullDT := IsBindlessLeveledDT <+ IsWFFull.
+Module Type IsBindlessLeveledFullDTWithLeibniz := IsBindlessLeveledDTWithLeibniz <+ IsWFFull.
 
 Module Type IsLvlDT := IsLeveledDT.
 Module Type IsLvlDTWL := IsLeveledDTWithLeibniz.
@@ -309,10 +265,10 @@ Module Type IsLeveledOTWithLeibniz := OrderedTypeWithLeibniz <+ IsLeveled.
 Module Type IsBindlessLeveledOT := Orders.OrderedType <+ IsBindlessLeveled.
 Module Type IsBindlessLeveledOTWithLeibniz := OrderedTypeWithLeibniz <+ IsBindlessLeveled.
 
-Module Type IsLeveledFullOT := IsLeveledOT <+ HasValidFull.
-Module Type IsLeveledFullOTWithLeibniz := IsLeveledOTWithLeibniz <+ HasValidFull.
-Module Type IsBindlessLeveledFullOT := IsBindlessLeveledOT <+ HasValidFull.
-Module Type IsBindlessLeveledFullOTWithLeibniz := IsBindlessLeveledOTWithLeibniz <+ HasValidFull.
+Module Type IsLeveledFullOT := IsLeveledOT <+ IsWFFull.
+Module Type IsLeveledFullOTWithLeibniz := IsLeveledOTWithLeibniz <+ IsWFFull.
+Module Type IsBindlessLeveledFullOT := IsBindlessLeveledOT <+ IsWFFull.
+Module Type IsBindlessLeveledFullOTWithLeibniz := IsBindlessLeveledOTWithLeibniz <+ IsWFFull.
 
 Module Type IsLvlOT := IsLeveledOT.
 Module Type IsLvlOTWL := IsLeveledOTWithLeibniz.
