theories/Set/SetLevelInterface.v
@@ -1,5 +1,5 @@
 From Coq Require Import MSets.
-From DeBrLevel Require Import LevelInterface SetOTwLInterface SetOTwL.
+From DeBrLevel Require Import LevelInterface Level SetOTwLInterface SetOTwL.
 
 (** * Interface - Leveled Set
 
@@ -8,14 +8,16 @@ From DeBrLevel Require Import LevelInterface SetOTwLInterface SetOTwL.
   between them and classical set operators such as ∈,∪, etc.
 
   [shift] is directly applied on elements of the set (like a map) and [valid] is satisfied 
-  by a set [s] under [k] only if all elements in [s] satisfy the validity property under [k]. 
+  by a set [t] under [n] only if all elements in [t] satisfy the validity property under [n]. 
 *)
 
-(** *** Leveled Set Interface with ordered elements with leibniz equality *)
+(** ** Leveled Set Interface - [OT] and [WL] *)
 Module Type IsLvlSetInterface 
-  (T : IsLvlOTWL) (Import St : SetOTWithLeibnizInterface T) <: IsLvlOTWL.
+            (T : IsLvlOTWL) (Import St : SetOTWithLeibnizInterface T) <: IsLvlOTWL.
 
 Include IsLvl St.
+
+(** *** Definitions *)
 
 Definition t := t.
 
@@ -31,66 +33,130 @@ Definition lt_compat := lt_compat.
 Definition compare := compare.
 Definition compare_spec := compare_spec.
 
-(** **** Valid 
-  [valid] is opaque outside, consequently we gives an explicit unfold lemma.
+(** *** Specifications *)
+Section specs.
+
+Variable m n : Lvl.t.
+Variable v : elt.
+Variable t t' : t.
+
+
+(** **** [Wf] specifications 
+  [Wf] is opaque outside, consequently we gives an explicit unfold lemma.
 *)
-Section valid.
 
-Variable lb : Lvl.t.
-Variable v : elt.
-Variable s s' : t.
+Parameter Wf_unfold : Wf m t <-> (For_all (T.Wf m) t).
+Parameter Wf_add_iff : Wf m (add v t) <-> T.Wf m v /\ Wf m t.
+Parameter Wf_empty : Wf m empty.
+Parameter Wf_union_iff : Wf m (union t t') <-> Wf m t /\ Wf m t'.
+Parameter Wf_singleton_iff : Wf m (singleton v) <-> T.Wf m v.
+Parameter Wf_in : Wf m t -> In v t -> T.Wf m v.
 
-Parameter valid_unfold : valid lb s <-> (For_all (T.valid lb) s).
-Parameter valid_add_spec : valid lb (add v s) -> T.valid lb v /\ valid lb s.
-Parameter valid_empty_spec : valid lb empty.
-Parameter valid_union_iff : valid lb (union s s') <-> valid lb s /\ valid lb s'.
-Parameter valid_singleton_iff : valid lb (singleton v) <-> T.valid lb v.
-Parameter valid_in_spec : valid lb s -> In v s -> T.valid lb v.
+(** **** [shift] specifications *)
 
-End valid.
+Parameter shift_Empty : Empty t -> shift m n t = empty.
+Parameter shift_empty : shift m n empty = empty.
+Parameter shift_singleton : shift m n (singleton v) = singleton (T.shift m n v).
+Parameter shift_union : shift m n (union t t') = union (shift m n t) (shift m n t').
+Parameter shift_inter : shift m n (inter t t') = inter (shift m n t) (shift m n t').
+Parameter shift_diff : shift m n (diff t t') = (diff (shift m n t) (shift m n t')).
 
-(** **** Shift *)
-Section shift.
+Parameter shift_add_notin :
+  ~ In v t -> shift m n (add v t) = add (T.shift m n v) (shift m n t).
+Parameter shift_add_in : In v t -> shift m n (add v t) = (shift m n t).
+Parameter shift_add : shift m n (add v t) = add (T.shift m n v) (shift m n t).
+Parameter shift_remove : shift m n (remove v t) = remove (T.shift m n v)(shift m n t).
 
-Variable lb k : Lvl.t.
-Variable v : elt.
-Variable s s' : t.
+Parameter shift_in_iff : In v t <-> In (T.shift m n v) (shift m n t).
+Parameter shift_in_e :
+  In v (shift m n t) -> 
+  exists v', v = (T.shift m n v') /\ In (T.shift m n v') (shift m n t).
+Parameter shift_notin_iff : ~ In v t <-> ~ In (T.shift m n v) (shift m n t).
 
-Parameter shift_Empty_spec : Empty s -> shift lb k s = empty.
-Parameter shift_empty_spec : shift lb k empty = empty.
-Parameter shift_singleton_spec : shift lb k (singleton v) = singleton (T.shift lb k v).
-Parameter shift_union_spec : shift lb k (union s s') = union (shift lb k s) (shift lb k s').
-Parameter shift_inter_spec : shift lb k (inter s s') = inter (shift lb k s) (shift lb k s').
-Parameter shift_diff_spec : shift lb k (diff s s') = (diff (shift lb k s) (shift lb k s')).
-
-Parameter shift_add_notin_spec :
-  ~ In v s -> shift lb k (add v s) = add (T.shift lb k v) (shift lb k s).
-Parameter shift_add_in_spec : In v s -> shift lb k (add v s) = (shift lb k s).
-Parameter shift_add_spec : shift lb k (add v s) = add (T.shift lb k v) (shift lb k s).
-Parameter shift_remove_spec : shift lb k (remove v s) = remove (T.shift lb k v)(shift lb k s).
-
-Parameter shift_in_iff : In v s <-> In (T.shift lb k v) (shift lb k s).
-Parameter shift_in_e_spec :
-  In v (shift lb k s) -> 
-  exists v', v = (T.shift lb k v') /\ In (T.shift lb k v') (shift lb k s).
-Parameter shift_notin_iff : ~ In v s <-> ~ In (T.shift lb k v) (shift lb k s).
-
-End shift.
+End specs.
 
 End IsLvlSetInterface.
 
+
 (** ---- *)
 
-(** *** Bindless Leveled Set Interface with ordered elements with leibniz equality *)
-Module Type IsBdlLvlSetInterface (T : IsLvlOTWL) (St : SetOTWithLeibnizInterface T) <: IsBdlLvlOTWL
-:= IsLvlSetInterface T St <+ IsBindlessLeveledEx.
+
+(** ** Leveled Set Interface - [OT], [BD] and [WL] *)
+Module Type IsBdlLvlSetInterface (T : IsLvlOTWL) (St : SetOTWithLeibnizInterface T) <: IsBdlLvlOTWL.
+
+Include IsLvlSetInterface T St.
+Import St.
+
+Parameter shift_wf_refl : forall (m n: Lvl.t) (t: t), Wf m t -> eq (shift m n t) t.
+Parameter Wf_in_iff : 
+  forall (m k: Lvl.t) (n: elt) (t: t), Wf m t -> In n (shift m k t) <-> In n t.
+
+End IsBdlLvlSetInterface.
 
 
-(** *** Leveled Set interface with boolean version of [valid] named [validb] *)
+(** ---- *)
+
+
+(** ** Leveled Set Interface - [OT], [FL] and [WL] *)
 Module Type IsLvlFullSetInterface (T : IsLvlFullOTWL) (St : SetOTWithLeibnizInterface T)
-:= (IsLvlSetInterface T St) <+ HasValidFull.
+:= (IsLvlSetInterface T St) <+ IsWFFull.
 
 
-(** *** Bindless Leveled Set interface with boolean version of [valid] named [validb] *)
+(** ---- *)
+
+
+(** ** Leveled Set Interface - [OT], [BD], [FL] and [WL] *)
 Module Type IsBdlLvlFullSetInterface (T : IsBdlLvlFullOTWL) (St : SetOTWithLeibnizInterface T)
-:= (IsBdlLvlSetInterface T St) <+ HasValidFull.
+:= (IsBdlLvlSetInterface T St) <+ IsWFFull.
+
+
+Module Type IsLvlSetLVLInterface (St: SetOTWithLeibnizInterface Level).
+
+Include IsBdlLvlFullSetInterface Level St.
+Import St.
+
+(** *** Definitions *)
+
+Parameter max_key : t -> Lvl.t.
+Parameter new_key : t -> Lvl.t.
+
+(** *** Specifications *)
+Section specifications.
+
+Variable m n k p: Lvl.t.
+Variable v : elt.
+Variable s s' : t.
+
+(** **** [max_key] specifications *)
+
+#[export] Declare Instance max_key_eq : Proper (eq ==> Logic.eq) max_key. 
+
+Parameter max_key_Empty : Empty s -> max_key s = 0.
+Parameter max_key_empty : max_key empty = 0.
+
+Parameter max_key_Add_max : Add v s s' -> max_key s' = max v (max_key s). 
+Parameter max_key_add_max : max_key (add v s) = max v (max_key s). 
+
+(** **** [new_key] specifications *)
+
+#[export] Declare Instance new_key_eq : Proper (eq ==> Logic.eq) new_key. 
+
+Parameter new_key_Empty : Empty s -> new_key s = 0.
+Parameter new_key_empty : new_key empty = 0.
+
+Parameter new_key_Add_max : Add v s s' -> new_key s' = max (S v) (new_key s). 
+Parameter new_key_add_max : new_key (add v s) = max (S v) (new_key s). 
+
+Parameter new_key_in_spec : In v s -> (v < new_key s)%nat.
+
+(** **** [shift] specifications *)
+
+Parameter shift_permute_1 :
+  eq (shift m n (shift m k s)) (shift (m + n) k (shift m n s)).
+
+Parameter shift_permute_2 :
+  m <= n -> eq (shift m k (shift n p s)) (shift (n + k) p (shift m k s)).
+
+End specifications.
+
+End IsLvlSetLVLInterface.
